Complete porting of automata definitions.

deps/poulet4/lib/P4automata/Benchmarks/SloppyStrict.v
@@ -18,7 +18,6 @@ Obligation Tactic := prep_equiv.
 
 
 Module Sloppy.
-
   Inductive state :=
   | ParseEthernet
   | ParseIPv4
@@ -27,86 +26,35 @@ Module Sloppy.
 
   Scheme Equality for state.
   Global Instance state_eqdec: EquivDec.EqDec state eq := state_eq_dec.
-
-  Global Program Instance state_finite: @Finite state _ state_eq_dec :=
-    {| enum := [ParseEthernet; ParseIPv4; ParseIPv6] |}.
-  Next Obligation.
-    repeat constructor;
-      repeat match goal with
-             | H: List.In _ [] |- _ => apply List.in_nil in H; exfalso; exact H
-             | |- ~ List.In _ [] => apply List.in_nil
-             | |- ~ List.In _ (_ :: _) => unfold not; intros
-             | H: List.In _ (_::_) |- _ => inversion H; clear H
-             | _ => discriminate
-             end.
-  Qed.
-  Next Obligation.
-    destruct x; intuition congruence.
-  Qed.
-
-  Inductive header : nat -> Type :=
-  | HdrEthernet : header 112
-  | HdrIPv4 : header 128
-  | HdrIPv6 : header 288
-  .
-
-  Definition h112_eq_dec (x y: header 112) : {x = y} + {x <> y} :=
-    match x, y with
-    | HdrEthernet, HdrEthernet => left eq_refl
-    | _, _ => idProp
-    end.
-
-  Definition h128_eq_dec (x y: header 128) : {x = y} + {x <> y} :=
-    match x, y with
-    | HdrIPv4, HdrIPv4 => left eq_refl
-    | _, _ => idProp
-    end.
-
-  Definition h288_eq_dec (x y: header 288) : {x = y} + {x <> y} :=
-    match x, y with
-    | HdrIPv6, HdrIPv6 => left eq_refl
-    | _, _ => idProp
-    end.
-
-  Definition header_eqdec_ (n: nat) (x: header n) (y: header n) : {x = y} + {x <> y}.
+  Global Instance state_finite: @Finite state _ state_eq_dec.
   Proof.
-    solve_header_eqdec_ n x y
-      ((existT (fun n => forall x y: header n, {x = y} + {x <> y}) _ h112_eq_dec) ::
-        (existT _ _ h128_eq_dec) :: (existT _ _ h288_eq_dec) :: nil).
+    solve_finiteness.
   Defined.
 
-  Global Instance header_eqdec: forall n, EquivDec.EqDec (header n) eq := header_eqdec_.
+  Inductive header :=
+  | HdrEthernet
+  | HdrIPv4
+  | HdrIPv6.
 
-  Global Instance header_eqdec': EquivDec.EqDec (Syntax.H' header) eq.
+  Definition sz (h: header): nat :=
+    match h with
+    | HdrEthernet => 112
+    | HdrIPv4 => 128
+    | HdrIPv6 => 288
+    end.
+
+  Scheme Equality for header.
+  Global Instance header_eqdec: EquivDec.EqDec header eq := header_eq_dec.
+  Global Instance header_finite: @Finite header _ header_eq_dec.
   Proof.
-    solve_eqdec'.
+    solve_finiteness.
   Defined.
 
-  Global Instance header_finite: forall n, @Finite (header n) _ _.
-  Proof.
-    intros n; solve_indexed_finiteness n [288; 128; 112].
-  Qed.
-
-  Global Program Instance header_finite': @Finite {n & header n} _ header_eqdec' :=
-    {| enum := [
-        existT _ _ HdrEthernet; existT _ _ HdrIPv4; existT _ _ HdrIPv6]; |}.
-  Next Obligation.
-    solve_header_finite.
-  Qed.
-  Next Obligation.
-  dependent destruction X; subst;
-  repeat (
-    match goal with
-    | |- ?L \/ ?R => (now left; trivial) || right
-    end
-  ).
-  Qed.
-
-  Definition states (s: state) :=
+  Definition states (s: state) : WP.P4A.state state sz :=
     match s with
     | ParseEthernet =>
       {| st_op := extract(HdrEthernet) ;
-         st_trans := transition select (| ESlice (EHdr HdrEthernet) 111 96 |) {{
+         st_trans := transition select (| ESlice _ (EHdr (sz := sz) HdrEthernet) 111 96 |) {{
            [| hexact 0x86dd |] ==> inl ParseIPv6 ;;;
             inl ParseIPv4
          }}
@@ -121,9 +69,9 @@ Module Sloppy.
       |}
     end.
 
-  Program Definition aut: Syntax.t state header :=
+  Program Definition aut: Syntax.t state sz :=
     {| t_states := states |}.
-  Solve Obligations with (destruct s; cbv; Lia.lia).
+  Solve Obligations with (destruct s || destruct h; cbv; Lia.lia).
 
 End Sloppy.
 
@@ -137,86 +85,35 @@ Module Strict.
 
   Scheme Equality for state.
   Global Instance state_eqdec: EquivDec.EqDec state eq := state_eq_dec.
-
-  Global Program Instance state_finite: @Finite state _ state_eq_dec :=
-    {| enum := [ParseEthernet; ParseIPv4; ParseIPv6] |}.
-  Next Obligation.
-    repeat constructor;
-      repeat match goal with
-             | H: List.In _ [] |- _ => apply List.in_nil in H; exfalso; exact H
-             | |- ~ List.In _ [] => apply List.in_nil
-             | |- ~ List.In _ (_ :: _) => unfold not; intros
-             | H: List.In _ (_::_) |- _ => inversion H; clear H
-             | _ => discriminate
-             end.
-  Qed.
-  Next Obligation.
-    destruct x; intuition congruence.
-  Qed.
-
-  Inductive header : nat -> Type :=
-  | HdrEthernet : header 112
-  | HdrIPv4 : header 128
-  | HdrIPv6 : header 288
-  .
-
-  Definition h112_eq_dec (x y: header 112) : {x = y} + {x <> y} :=
-    match x, y with
-    | HdrEthernet, HdrEthernet => left eq_refl
-    | _, _ => idProp
-    end.
-
-  Definition h128_eq_dec (x y: header 128) : {x = y} + {x <> y} :=
-    match x, y with
-    | HdrIPv4, HdrIPv4 => left eq_refl
-    | _, _ => idProp
-    end.
-
-  Definition h288_eq_dec (x y: header 288) : {x = y} + {x <> y} :=
-    match x, y with
-    | HdrIPv6, HdrIPv6 => left eq_refl
-    | _, _ => idProp
-    end.
-
-  Definition header_eqdec_ (n: nat) (x: header n) (y: header n) : {x = y} + {x <> y}.
+  Global Instance state_finite: @Finite state _ state_eq_dec.
   Proof.
-    solve_header_eqdec_ n x y
-      ((existT (fun n => forall x y: header n, {x = y} + {x <> y}) _ h112_eq_dec) ::
-        (existT _ _ h128_eq_dec) :: (existT _ _ h288_eq_dec) :: nil).
+    solve_finiteness.
   Defined.
 
-  Global Instance header_eqdec: forall n, EquivDec.EqDec (header n) eq := header_eqdec_.
+  Inductive header :=
+  | HdrEthernet
+  | HdrIPv4
+  | HdrIPv6.
 
-  Global Instance header_eqdec': EquivDec.EqDec (Syntax.H' header) eq.
+  Definition sz (h: header): nat :=
+    match h with
+    | HdrEthernet => 112
+    | HdrIPv4 => 128
+    | HdrIPv6 => 288
+    end.
+
+  Scheme Equality for header.
+  Global Instance header_eqdec: EquivDec.EqDec header eq := header_eq_dec.
+  Global Instance header_finite: @Finite header _ header_eq_dec.
   Proof.
-    solve_eqdec'.
+    solve_finiteness.
   Defined.
 
-  Global Instance header_finite: forall n, @Finite (header n) _ _.
-  Proof.
-    intros n; solve_indexed_finiteness n [288; 128; 112].
-  Qed.
-
-  Global Program Instance header_finite': @Finite {n & header n} _ header_eqdec' :=
-    {| enum := [
-        existT _ _ HdrEthernet; existT _ _ HdrIPv4; existT _ _ HdrIPv6]; |}.
-  Next Obligation.
-    solve_header_finite.
-  Qed.
-  Next Obligation.
-  dependent destruction X; subst;
-  repeat (
-    match goal with
-    | |- ?L \/ ?R => (now left; trivial) || right
-    end
-  ).
-  Qed.
-
-  Definition states (s: state) :=
+  Definition states (s: state) : WP.P4A.state state sz :=
     match s with
     | ParseEthernet =>
       {| st_op := extract(HdrEthernet) ;
-         st_trans := transition select (| ESlice (EHdr HdrEthernet) 111 96 |) {{
+         st_trans := transition select (| ESlice _ (EHdr HdrEthernet) 111 96 |) {{
            [| hexact 0x86dd |] ==> inl ParseIPv6 ;;;
            [| hexact 0x8600 |] ==> inl ParseIPv4 ;;;
             reject
@@ -232,9 +129,9 @@ Module Strict.
       |}
     end.
 
-  Program Definition aut: Syntax.t state header :=
+  Program Definition aut: Syntax.t state sz :=
     {| t_states := states |}.
-  Solve Obligations with (destruct s; cbv; Lia.lia).
+  Solve Obligations with (destruct s || destruct h; cbv; Lia.lia).
 
 End Strict.
 
