deps/poulet4/lib/P4automata/Benchmarks/SmallFilter.v
@@ -19,68 +19,32 @@ Module IncrementalBits.
   Inductive state :=
   | Start
   | Finish.
+
   Scheme Equality for state.
   Global Instance state_eqdec: EquivDec.EqDec state eq := state_eq_dec.
-  Global Program Instance state_finite: @Finite state _ state_eq_dec :=
-    {| enum := [Start; Finish] |}.
-  Next Obligation.
-    repeat constructor;
-      repeat match goal with
-             | H: List.In _ [] |- _ => apply List.in_nil in H; exfalso; exact H
-             | |- ~ List.In _ [] => apply List.in_nil
-             | |- ~ List.In _ (_ :: _) => unfold not; intros
-             | H: List.In _ (_::_) |- _ => inversion H; clear H
-             | _ => discriminate
-             end.
-  Qed.
-  Next Obligation.
-    destruct x; intuition congruence.
-  Qed.
-
-  Inductive header : nat -> Type :=
-  | Pref : header 1
-  | Suf : header 1.
-
-  Derive Signature for header.
-
-  Equations header_eqdec_ (n: nat) (x: IncrementalBits.header n) (y: IncrementalBits.header n) : {x = y} + {x <> y} :=
-  {
-    header_eqdec_ _ IncrementalBits.Pref IncrementalBits.Pref := left eq_refl ;
-    header_eqdec_ _ IncrementalBits.Suf IncrementalBits.Suf := left eq_refl ;
-    header_eqdec_ _ _ _ := ltac:(right; congruence) ;
-  }.
-
-  Global Instance header_eqdec: forall n, EquivDec.EqDec (header n) eq := header_eqdec_.
-
-  Global Instance header_eqdec': EquivDec.EqDec (Syntax.H' header) eq.
+  Global Instance state_finite: @Finite state _ state_eq_dec.
   Proof.
-    solve_eqdec'.
+    solve_finiteness.
   Defined.
 
-  Global Instance header_finite: forall n, @Finite (header n) _ _.
+  Inductive header :=
+  | Pref : header
+  | Suf : header.
+
+  Definition sz (h: header): nat :=
+    match h with
+    | Pref
+    | Suf => 1
+    end.
+
+  Scheme Equality for header.
+  Global Instance header_eqdec: EquivDec.EqDec header eq := header_eq_dec.
+  Global Instance header_finite: @Finite header _ header_eq_dec.
   Proof.
-    intros n; solve_indexed_finiteness n [1; 1].
-  Qed.
+    solve_finiteness.
+  Defined.
 
-  Global Program Instance header_finite': @Finite {n & header n} _ header_eqdec' :=
-    {| enum := [ existT _ _ Pref ; existT _ _ Suf] |}.
-  Next Obligation.
-    repeat constructor;
-    unfold "~";
-    intros;
-    destruct H;
-    now inversion H || now inversion H0.
-  Qed.
-  Next Obligation.
-  dependent destruction X; subst;
-  repeat (
-    match goal with
-    | |- ?L \/ ?R => (now left; trivial) || right
-    end
-  ).
-  Qed.
-
-  Definition states (s: state) :=
+  Definition states (s: state) : Syntax.state state sz :=
     match s with
     | Start =>
       {| st_op := extract(Pref);
@@ -94,79 +58,42 @@ Module IncrementalBits.
          st_trans := transition accept |}
     end.
 
-  Program Definition aut: Syntax.t state header :=
+  Program Definition aut: Syntax.t state sz :=
     {| t_states := states |}.
-  Solve Obligations with (destruct s; cbv; Lia.lia).
+  Solve Obligations with (destruct s || destruct h; cbv; Lia.lia).
 
 End IncrementalBits.
 
 Module BigBits.
   Inductive state :=
   | Parse.
-  Global Instance state_eqdec: EquivDec.EqDec state eq.
-  vm_compute.
-  intros.
-  left.
-  destruct x; destruct x0; trivial.
-  Defined.
-  Global Program Instance state_finite: @Finite state _ state_eqdec :=
-    {| enum := [Parse] |}.
-  Next Obligation.
-    repeat constructor;
-      repeat match goal with
-             | H: List.In _ [] |- _ => apply List.in_nil in H; exfalso; exact H
-             | |- ~ List.In _ [] => apply List.in_nil
-             | |- ~ List.In _ (_ :: _) => unfold not; intros
-             | H: List.In _ (_::_) |- _ => inversion H; clear H
-             | _ => discriminate
-             end.
-  Qed.
-  Next Obligation.
-    destruct x; intuition congruence.
-  Qed.
 
-  Inductive header : nat -> Type :=
-  | Pref : header 1
-  | Suf : header 1.
-
-  Equations header_eqdec_ (n: nat) (x: BigBits.header n) (y: BigBits.header n) : {x = y} + {x <> y} :=
-  {
-    header_eqdec_ _ BigBits.Pref BigBits.Pref := left eq_refl ;
-    header_eqdec_ _ BigBits.Suf BigBits.Suf := left eq_refl ;
-    header_eqdec_ _ _ _ := ltac:(right; congruence) ;
-  }.
-
-  Global Instance header_eqdec: forall n, EquivDec.EqDec (header n) eq := header_eqdec_.
-
-  Global Instance header_finite: forall n, @Finite (header n) _ (header_eqdec n).
+  Equations state_eq_dec (h1 h2: state) : {h1 = h2} + {h1 <> h2} :=
+  { state_eq_dec Parse Parse := left eq_refl }.
+  Global Instance state_eqdec: EquivDec.EqDec state eq := state_eq_dec.
+  Global Instance state_finite: @Finite state _ state_eq_dec.
   Proof.
-    intros n; solve_indexed_finiteness n [1; 1].
-  Qed.
-
-  Global Instance header_eqdec': EquivDec.EqDec {n & header n} eq.
-  Proof.
-    solve_eqdec'.
+    solve_finiteness.
   Defined.
 
-  Global Program Instance header_finite': @Finite {n & header n} _ header_eqdec' :=
-    {| enum := [ existT _ _ Pref ; existT _ _ Suf] |}.
-  Next Obligation.
-    repeat constructor;
-    unfold "~";
-    intros;
-    destruct H;
-    now inversion H || now inversion H0.
-  Qed.
-  Next Obligation.
-  dependent destruction X; subst;
-  repeat (
-    match goal with
-    | |- ?L \/ ?R => (now left; trivial) || right
-    end
-  ).
-  Qed.
+  Inductive header :=
+  | Pref : header
+  | Suf : header.
 
-  Definition states (s: state) :=
+  Scheme Equality for header.
+  Global Instance header_eqdec: EquivDec.EqDec header eq := header_eq_dec.
+  Global Instance header_finite: @Finite header _ header_eq_dec.
+  Proof.
+    solve_finiteness.
+  Defined.
+
+  Definition sz (h: header): nat :=
+    match h with
+    | Pref
+    | Suf => 1
+    end.
+
+  Definition states (s: state) : Syntax.state state sz :=
     match s with
     | Parse =>
       {| st_op :=
@@ -179,211 +106,67 @@ Module BigBits.
       |}
     end.
 
-  Program Definition aut: Syntax.t state header :=
+  Program Definition aut: Syntax.t state sz :=
     {| t_states := states |}.
-  Solve Obligations with (destruct s; cbv; Lia.lia).
+  Solve Obligations with (destruct s || destruct h; cbv; Lia.lia).
 
 End BigBits.
 
 Module OneBit.
   Inductive state :=
   | Parse.
-  Global Instance state_eqdec: EquivDec.EqDec state eq.
-  vm_compute.
-  intros.
-  left.
-  destruct x; destruct x0; trivial.
-  Defined.
-  Global Program Instance state_finite: @Finite state _ state_eqdec :=
-    {| enum := [Parse] |}.
-  Next Obligation.
-    repeat constructor;
-      repeat match goal with
-             | H: List.In _ [] |- _ => apply List.in_nil in H; exfalso; exact H
-             | |- ~ List.In _ [] => apply List.in_nil
-             | |- ~ List.In _ (_ :: _) => unfold not; intros
-             | H: List.In _ (_::_) |- _ => inversion H; clear H
-             | _ => discriminate
-             end.
-  Qed.
-  Next Obligation.
-    destruct x; intuition congruence.
-  Qed.
 
-  Inductive header : nat -> Type :=
-  | Pref : header 2.
-
-  Global Instance header_eqdec: forall n, EquivDec.EqDec (header n) eq.
+  Equations state_eq_dec (h1 h2: state) : {h1 = h2} + {h1 <> h2} :=
+  { state_eq_dec Parse Parse := left eq_refl }.
+  Global Instance state_eqdec: EquivDec.EqDec state eq := state_eq_dec.
+  Global Instance state_finite: @Finite state _ state_eq_dec.
   Proof.
-    solve_eqdec.
+    solve_finiteness.
   Defined.
 
-  Global Instance header_finite: forall n, @Finite (header n) _ (header_eqdec n).
-  Proof.
-    intros n; solve_indexed_finiteness n [2].
-  Qed.
+  Inductive header :=
+  | Pref : header.
 
-  Global Instance header_eqdec': EquivDec.EqDec {n & header n} eq.
+  Equations header_eq_dec (h1 h2: header) : {h1 = h2} + {h1 <> h2} :=
+  { header_eq_dec Pref Pref := left eq_refl }.
+  Global Instance header_eqdec: EquivDec.EqDec header eq := header_eq_dec.
+  Global Instance header_finite: @Finite header _ header_eq_dec.
   Proof.
-    solve_eqdec'.
+    solve_finiteness.
   Defined.
 
-  Global Program Instance header_finite': @Finite {n & header n} _ header_eqdec' :=
-    {| enum := [ existT _ _ Pref ] |}.
-  Next Obligation.
-    repeat constructor;
-    unfold "~";
-    intros;
-    destruct H;
-    now inversion H || now inversion H0.
-  Qed.
-  Next Obligation.
-  dependent destruction X; subst;
-  repeat (
-    match goal with
-    | |- ?L \/ ?R => (now left; trivial) || right
-    end
-  ).
-  Qed.
+  Definition sz (h: header): nat :=
+    match h with
+    | Pref => 2
+    end.
 
-  Definition states (s: state) :=
+  Definition states (s: state) : Syntax.state state sz :=
     match s with
     | Parse =>
       {| st_op := extract(Pref);
-         st_trans := transition select (| (EHdr Pref)[0 -- 0] |) {{
+         st_trans := transition select (| (EHdr (sz := sz) Pref)[0 -- 0] |) {{
            [| exact #b|1 |] ==> accept ;;;
             @reject state
          }}
       |}
     end.
 
-  Program Definition aut: Syntax.t state header :=
+  Program Definition aut: Syntax.t state sz :=
     {| t_states := states |}.
-  Solve Obligations with (destruct s; cbv; Lia.lia).
+  Solve Obligations with (destruct s || destruct h; cbv; Lia.lia).
 
 End OneBit.
 
 Module IncrementalSeparate.
-
-  Definition state: Type := IncrementalBits.state + BigBits.state.
-  Global Instance state_eq_dec: EquivDec.EqDec state eq :=
-    ltac:(typeclasses eauto).
-
-  Definition header := Sum.H IncrementalBits.header BigBits.header.
-  Global Instance header_eq_dec': EquivDec.EqDec (H' header) eq.
-  Proof.
-    eapply Sum.H'_eq_dec; typeclasses eauto.
-  Defined.
-
-  Global Instance header_eq_dec: forall n, EquivDec.EqDec (header n) eq.
-  Proof.
-    typeclasses eauto.
-  Defined.
-
-  Global Instance header_finite: forall n, @Finite (header n) _ (header_eq_dec n).
-  Proof.
-    typeclasses eauto.
-  Defined.
-
-  Global Instance header_finite': @Finite {n & header n} _ header_eq_dec'.
-  econstructor.
-  - eapply Sum.H_finite.
-  - intros.
-    simpl.
-    destruct x.
-    inversion h;
-    dependent destruction H;
-    dependent destruction h;
-    dependent destruction h;
-    repeat (
-      match goal with
-      | |- ?L \/ ?R => (now left; trivial) || right
-      end
-    ).
-  Defined.
-
   Definition aut := Sum.sum IncrementalBits.aut BigBits.aut.
 End IncrementalSeparate.
 
 Module SeparateCombined.
-  Definition state: Type := BigBits.state + OneBit.state.
-  Global Instance state_eq_dec: EquivDec.EqDec state eq :=
-    ltac:(typeclasses eauto).
-
-  Definition header := Sum.H BigBits.header OneBit.header.
-  Global Instance header_eq_dec': EquivDec.EqDec (H' header) eq.
-  Proof.
-    eapply Sum.H'_eq_dec; typeclasses eauto.
-  Defined.
-
-  Global Instance header_eq_dec: forall n, EquivDec.EqDec (header n) eq.
-  Proof.
-    typeclasses eauto.
-  Defined.
-
-  Global Instance header_finite: forall n, @Finite (header n) _ (header_eq_dec n).
-  Proof.
-    typeclasses eauto.
-  Defined.
-
-  Global Instance header_finite': @Finite {n & header n} _ header_eq_dec'.
-  econstructor.
-  - eapply Sum.H_finite.
-  - intros.
-    simpl.
-    destruct x.
-    inversion h;
-    dependent destruction H;
-    dependent destruction h;
-    dependent destruction h;
-    repeat (
-      match goal with
-      | |- ?L \/ ?R => (now left; trivial) || right
-      end
-    ).
-  Defined.
-
   Definition aut := Sum.sum BigBits.aut OneBit.aut.
 End SeparateCombined.
 
 Module IncrementalCombined.
-  Definition state: Type := IncrementalBits.state + OneBit.state.
-  Global Instance state_eq_dec: EquivDec.EqDec state eq :=
-    ltac:(typeclasses eauto).
-
-  Definition header := Sum.H IncrementalBits.header OneBit.header.
-  Global Instance header_eq_dec': EquivDec.EqDec (H' header) eq.
-  Proof.
-    eapply Sum.H'_eq_dec; typeclasses eauto.
-  Defined.
-
-  Global Instance header_eq_dec: forall n, EquivDec.EqDec (header n) eq.
-  Proof.
-    typeclasses eauto.
-  Defined.
-
-  Global Instance header_finite: forall n, @Finite (header n) _ (header_eq_dec n).
-  Proof.
-    typeclasses eauto.
-  Defined.
-
-  Global Instance header_finite': @Finite {n & header n} _ header_eq_dec'.
-  econstructor.
-  - eapply Sum.H_finite.
-  - intros.
-    simpl.
-    destruct x.
-    inversion h;
-    dependent destruction H;
-    dependent destruction h;
-    dependent destruction h;
-    repeat (
-      match goal with
-      | |- ?L \/ ?R => (now left; trivial) || right
-      end
-    ).
-  Defined.
-
+  Definition aut := Sum.sum IncrementalBits.aut OneBit.aut.
 End IncrementalCombined.
 
 
