deps/poulet4/lib/P4automata/Benchmarks/TLVSmall.v
@@ -11,13 +11,6 @@ Require Import Poulet4.P4automata.BisimChecker.
 
 Open Scope p4a.
 
-Ltac prep_equiv :=
-  unfold Equivalence.equiv, RelationClasses.complement in *;
-  program_simpl; try congruence.
-
-Obligation Tactic := prep_equiv.
-
-
 Module TLVRefSmall.
   Inductive state :=
   | Parse1
@@ -34,170 +27,45 @@ Module TLVRefSmall.
   | Parse33.
 
   Scheme Equality for state.
-
   Global Instance state_eqdec: EquivDec.EqDec state eq := state_eq_dec.
-  Global Program Instance state_finite: @Finite state _ state_eq_dec :=
-    {| enum := [Parse1; Parse2; Parse3;
-        Parse11; Parse21; Parse31; 
-        Parse12; Parse22; Parse32; 
-        Parse13; Parse23; Parse33
-        ]; |}.
-  Next Obligation.
-    repeat constructor;
-      repeat match goal with
-             | H: List.In _ [] |- _ => apply List.in_nil in H; exfalso; exact H
-             | |- ~ List.In _ [] => apply List.in_nil
-             | |- ~ List.In _ (_ :: _) => unfold not; intros
-             | H: List.In _ (_::_) |- _ => inversion H; clear H
-             | _ => discriminate
-             end.
-  Qed.
-  Next Obligation.
-    destruct x; intuition congruence.
-  Qed.
-
-  Inductive header : nat -> Type :=
-  | Scratch8 : header 8
-  | Scratch16 : header 16
-  | T1 : header 6
-  | L1 : header 2
-  | V1 : header 24
-  | T2 : header 6
-  | L2 : header 2
-  | V2 : header 24
-  | T3 : header 6
-  | L3 : header 2
-  | V3 : header 24.
-
-  Derive Signature for header.
-
-  Definition h2_eq_dec (x y: header 2) : {x = y} + {x <> y}.
-    refine (
-    match x with 
-    | L1 => 
-      match y with 
-      | L1 => left eq_refl
-      | L2 => right _
-      | L3 => right _
-      end
-    | L2 => 
-      match y with 
-      | L1 => right _
-      | L2 => left eq_refl
-      | L3 => right _
-      end
-    | L3 => 
-      match y with 
-      | L1 => right _
-      | L2 => right _
-      | L3 => left eq_refl
-      end
-    end
-  ); intros H; inversion H.
-  Defined.
-
-  Definition h6_eq_dec (x y: header 6) : {x = y} + {x <> y}.
-    refine (
-    match x with 
-    | T1 => 
-      match y with 
-      | T1 => left eq_refl
-      | T2 => right _
-      | T3 => right _
-      end
-    | T2 => 
-      match y with 
-      | T1 => right _
-      | T2 => left eq_refl
-      | T3 => right _
-      end
-    | T3 => 
-      match y with 
-      | T1 => right _
-      | T2 => right _
-      | T3 => left eq_refl
-      end
-    end
-  ); intros H; inversion H.
-  Defined.
-
-  Definition h8_eq_dec (x y: header 8) : {x = y} + {x <> y} :=
-    match x, y with 
-    | Scratch8, Scratch8 => left eq_refl
-    | _, _ => idProp
-    end.
-
-  Definition h16_eq_dec (x y: header 16) : {x = y} + {x <> y} :=
-    match x, y with 
-    | Scratch16, Scratch16 => left eq_refl
-    | _, _ => idProp
-    end.
-
-  Definition h24_eq_dec (x y: header 24) : {x = y} + {x <> y}.
-    refine (
-    match x with 
-    | V1 => 
-      match y with 
-      | V1 => left eq_refl
-      | V2 => right _
-      | V3 => right _
-      end
-    | V2 => 
-      match y with 
-      | V1 => right _
-      | V2 => left eq_refl
-      | V3 => right _
-      end
-    | V3 => 
-      match y with 
-      | V1 => right _
-      | V2 => right _
-      | V3 => left eq_refl
-      end
-    end
-  ); intros H; inversion H.
-  Defined.
-
-  Definition header_eqdec_ (n: nat) (x: header n) (y: header n) : {x = y} + {x <> y}.
-    solve_header_eqdec_ n x y 
-      ((existT (fun n => forall x y: header n, {x = y} + {x <> y}) _ h2_eq_dec) :: 
-        (existT _ _ h6_eq_dec) :: (existT _ _ h8_eq_dec) :: (existT _ _ h16_eq_dec) :: (existT _ _ h24_eq_dec) :: nil).
-  Defined. 
-
-  Global Instance header_eqdec: forall n, EquivDec.EqDec (header n) eq := header_eqdec_.
-
-  Global Instance header_eqdec': EquivDec.EqDec (Syntax.H' header) eq.
+  Global Instance state_finite: @Finite state _ state_eq_dec.
   Proof.
-    solve_eqdec'.
+    solve_finiteness.
   Defined.
 
-  Global Instance header_finite: forall n, @Finite (header n) _ _.
-  Proof.
-    intros n; solve_indexed_finiteness n [24; 16; 8; 6; 2].
-  Qed.
+  Inductive header :=
+  | Scratch8
+  | Scratch16
+  | T1
+  | L1
+  | V1
+  | T2
+  | L2
+  | V2
+  | T3
+  | L3
+  | V3.
 
-  Global Program Instance header_finite': @Finite {n & header n} _ header_eqdec' :=
-    {| enum := [ 
-        existT _ _ Scratch8; existT _ _ Scratch16; 
-        existT _ _ T1; existT _ _ L1;  existT _ _ V1;
-        existT _ _ T2; existT _ _ L2;  existT _ _ V2;
-        existT _ _ T3; existT _ _ L3;  existT _ _ V3]; |}.
-  Next Obligation.
-    solve_header_finite.
-  Qed.
-  Next Obligation.
-  dependent destruction X; subst;
-  repeat (
-    match goal with
-    | |- ?L \/ ?R => (now left; trivial) || right
-    end
-  ).
-  Qed.
+  Scheme Equality for header.
+  Global Instance header_eqdec: EquivDec.EqDec header eq := header_eq_dec.
+  Global Instance header_finite: @Finite header _ header_eq_dec.
+  Proof.
+    solve_finiteness.
+  Defined.
+
+  Definition sz (h: header): nat :=
+    match h with
+    | Scratch8 => 8
+    | Scratch16 => 16
+    | T1 | T2 | T3 => 6
+    | L1 | L2 | L3 => 2
+    | V1 | V2 | V3 => 24
+    end.
 
   Definition states (s: state) :=
     match s with
     | Parse1 =>
-      {| st_op := 
+      {| st_op :=
           extract(T1) ;;
           extract(L1) ;
          st_trans := transition select (| EHdr T1, EHdr L1 |) {{
@@ -210,15 +78,15 @@ Module TLVRefSmall.
          }}
       |}
     | Parse11 =>
-      {| st_op := 
+      {| st_op :=
           extract(Scratch8) ;;
-          V1 <- EConcat (m := 16) (EHdr Scratch8) ((EHdr V1)[24--8]); 
+          V1 <- EConcat (m := 16) (EHdr Scratch8) ((EHdr (sz := sz) V1)[24--8]);
          st_trans := transition (inl Parse2)
       |}
     | Parse12 =>
-      {| st_op := 
+      {| st_op :=
           extract(Scratch16) ;;
-          V1 <- EConcat (m := 8) (EHdr Scratch16) ((EHdr V1)[24--16]); 
+          V1 <- EConcat (m := 8) (EHdr Scratch16) ((EHdr (sz := sz) V1)[24--16]);
          st_trans := transition (inl Parse2)
       |}
     | Parse13 =>
@@ -227,7 +95,7 @@ Module TLVRefSmall.
       |}
 
     | Parse2 =>
-      {| st_op := 
+      {| st_op :=
           extract(T2) ;;
           extract(L2) ;
          st_trans := transition select (| EHdr T2, EHdr L2 |) {{
@@ -240,15 +108,15 @@ Module TLVRefSmall.
          }}
       |}
     | Parse21 =>
-      {| st_op := 
+      {| st_op :=
           extract(Scratch8) ;;
-          V1 <- EConcat (m := 16) (EHdr Scratch8) ((EHdr V2)[24--8]); 
+          V1 <- EConcat (m := 16) (EHdr Scratch8) ((EHdr (sz := sz) V2)[24--8]);
          st_trans := transition (inl Parse3)
       |}
     | Parse22 =>
-      {| st_op := 
+      {| st_op :=
           extract(Scratch16) ;;
-          V1 <- EConcat (m := 8) (EHdr Scratch16) ((EHdr V2)[24--16]); 
+          V1 <- EConcat (m := 8) (EHdr Scratch16) ((EHdr (sz := sz) V2)[24--16]);
          st_trans := transition (inl Parse3)
       |}
     | Parse23 =>
@@ -257,7 +125,7 @@ Module TLVRefSmall.
       |}
 
     | Parse3 =>
-      {| st_op := 
+      {| st_op :=
           extract(T3) ;;
           extract(L3) ;
          st_trans := transition select (| EHdr T3, EHdr L3 |) {{
@@ -270,15 +138,15 @@ Module TLVRefSmall.
          }}
       |}
     | Parse31 =>
-      {| st_op := 
+      {| st_op :=
           extract(Scratch8) ;;
-          V1 <- EConcat (m := 16) (EHdr Scratch8) ((EHdr V3)[24--8]); 
+          V1 <- EConcat (m := 16) (EHdr Scratch8) ((EHdr (sz := sz) V3)[24--8]);
          st_trans := transition accept
       |}
     | Parse32 =>
-      {| st_op := 
+      {| st_op :=
           extract(Scratch16) ;;
-          V1 <- EConcat (m := 8) (EHdr Scratch16) ((EHdr V3)[24--16]); 
+          V1 <- EConcat (m := 8) (EHdr Scratch16) ((EHdr (sz := sz) V3)[24--16]);
          st_trans := transition accept
       |}
     | Parse33 =>
@@ -287,9 +155,9 @@ Module TLVRefSmall.
       |}
     end.
 
-  Program Definition aut: Syntax.t state header :=
+  Program Definition aut: Syntax.t state sz :=
     {| t_states := states |}.
-  Solve Obligations with (destruct s; cbv; Lia.lia).
+  Solve Obligations with (destruct s || destruct h; cbv; Lia.lia).
 
 End TLVRefSmall.
 
