deps/poulet4/lib/P4automata/Benchmarks/Timestamp.v
@@ -28,134 +28,45 @@ Module TimestampRefKeepSingle.
   | ParseValue6.
 
   Scheme Equality for state.
-
   Global Instance state_eqdec: EquivDec.EqDec state eq := state_eq_dec.
-  Global Program Instance state_finite: @Finite state _ state_eq_dec :=
-    {| enum := [Start; ParseValue1; ParseValue2; ParseValue3; ParseValue4; ParseValue5; ParseValue6] |}.
-  Next Obligation.
-    repeat constructor;
-      repeat match goal with
-            | H: List.In _ [] |- _ => apply List.in_nil in H; exfalso; exact H
-            | |- ~ List.In _ [] => apply List.in_nil
-            | |- ~ List.In _ (_ :: _) => unfold not; intros
-            | H: List.In _ (_::_) |- _ => inversion H; clear H
-            | _ => discriminate
-            end.
-  Qed.
-  Next Obligation.
-    destruct x; intuition congruence.
-  Qed.
-
-  Inductive header : nat -> Type :=
-  | Typ : header 8
-  | Len : header 8
-  | Value : header 48
-  | Scratch8 : header 8
-  | Scratch16 : header 16
-  | Scratch24 : header 24
-  | Scratch32 : header 32
-  | Scratch40 : header 40.
-
-  Derive Signature for header.
-
-  Definition h16_eq_dec (x y: header 16) : {x = y} + {x <> y} :=
-    match x, y with 
-    | Scratch16, Scratch16 => left eq_refl
-    | _, _ => idProp
-    end.
-
-  Definition h24_eq_dec (x y: header 24) : {x = y} + {x <> y} :=
-    match x, y with 
-    | Scratch24, Scratch24 => left eq_refl
-    | _, _ => idProp
-    end.
-
-  Definition h32_eq_dec (x y: header 32) : {x = y} + {x <> y} :=
-    match x, y with 
-    | Scratch32, Scratch32 => left eq_refl
-    | _, _ => idProp
-    end.
-
-  Definition h40_eq_dec (x y: header 40) : {x = y} + {x <> y} :=
-    match x, y with 
-    | Scratch40, Scratch40 => left eq_refl
-    | _, _ => idProp
-    end.
-
-  Definition h48_eq_dec (x y: header 48) : {x = y} + {x <> y} :=
-    match x, y with 
-    | Value, Value => left eq_refl
-    | _, _ => idProp
-    end.
-
-  Definition h8_eq_dec (x y: header 8) : {x = y} + {x <> y}. 
-  refine (
-    match x with 
-    | Typ => 
-      match y with 
-      | Typ => left eq_refl
-      | Len => right _
-      | Scratch8 => right _
-      end
-    | Len => 
-      match y with 
-      | Typ => right _
-      | Len => left eq_refl
-      | Scratch8 => right _
-      end
-    | Scratch8 => 
-        match y with 
-        | Typ => right _
-        | Len => right _
-        | Scratch8 => left eq_refl
-        end
-    end
-  ); unfold "<>"; intros H; inversion H.
+  Global Instance state_finite: @Finite state _ state_eq_dec.
+  Proof.
+    solve_finiteness.
   Defined.
 
+  Inductive header :=
+  | Typ
+  | Len
+  | Value
+  | Scratch8
+  | Scratch16
+  | Scratch24
+  | Scratch32
+  | Scratch40.
 
-  Definition header_eqdec_ (n: nat) (x: header n) (y: header n) : {x = y} + {x <> y}.
-    solve_header_eqdec_ n x y 
-      ((existT (fun n => forall x y: header n, {x = y} + {x <> y}) _ h8_eq_dec) :: 
-        (existT _ _ h16_eq_dec) :: (existT _ _ h24_eq_dec) :: (existT _ _ h32_eq_dec) :: 
-        (existT _ _ h40_eq_dec) :: (existT _ _ h48_eq_dec) :: nil).
-  Defined. 
-
-  Global Instance header_eqdec: forall n, EquivDec.EqDec (header n) eq := header_eqdec_.
-
-  Global Instance header_eqdec': EquivDec.EqDec (Syntax.H' header) eq.
+  Scheme Equality for header.
+  Global Instance header_eqdec: EquivDec.EqDec header eq := header_eq_dec.
+  Global Instance header_finite: @Finite header _ header_eq_dec.
   Proof.
-    solve_eqdec'.
+    solve_finiteness.
   Defined.
 
-  Global Instance header_finite: forall n, @Finite (header n) _ _.
-  Proof.
-    intros n; solve_indexed_finiteness n [8; 16; 24; 32; 40; 48].
-  Qed.
+  Definition sz (h: header): nat :=
+    match h with
+    | Typ => 8
+    | Len => 8
+    | Value => 48
+    | Scratch8 => 8
+    | Scratch16 => 16
+    | Scratch24 => 24
+    | Scratch32 => 32
+    | Scratch40 => 40
+    end.
 
-  Global Program Instance header_finite': @Finite {n & header n} _ header_eqdec' :=
-    {| enum := [ 
-      existT _ _ Len; existT _ _ Typ; existT _ _ Value;  
-      existT _ _ Scratch8; existT _ _ Scratch16; existT _ _ Scratch24;
-      existT _ _ Scratch32; existT _ _ Scratch40
-      
-      ] |}.
-  Next Obligation.
-    solve_header_finite.
-  Qed.
-  Next Obligation.
-  dependent destruction X; subst;
-  repeat (
-    match goal with
-    | |- ?L \/ ?R => (now left; trivial) || right
-    end
-  ).
-  Qed.
-
-  Definition states (s: state) :=
+  Definition states (s: state) : Syntax.state state sz :=
     match s with
     | Start =>
-      {| st_op := 
+      {| st_op :=
           extract(Typ) ;;
           extract(Len) ;
         st_trans := transition select (| EHdr Len |) {{
@@ -170,33 +81,33 @@ Module TimestampRefKeepSingle.
         }}
       |}
     | ParseValue1 =>
-      {| st_op := 
-          extract(Scratch8) ;; 
-          Value <- EConcat (m := 40) (EHdr Scratch8) ((EHdr Value)[48--8])  ;
+      {| st_op :=
+          extract(Scratch8) ;;
+          Value <- EConcat (m := 40) (EHdr Scratch8) ((EHdr (sz := sz) Value)[48--8])  ;
         st_trans := transition accept
       |}
     | ParseValue2 =>
-      {| st_op := 
-          extract(Scratch16) ;; 
-          Value <- EConcat (m := 32) (EHdr Scratch16) ((EHdr Value)[48--16])  ;
+      {| st_op :=
+          extract(Scratch16) ;;
+          Value <- EConcat (m := 32) (EHdr Scratch16) ((EHdr (sz := sz) Value)[48--16])  ;
         st_trans := transition accept
       |}
     | ParseValue3 =>
-      {| st_op := 
-          extract(Scratch24) ;; 
-          Value <- EConcat (m := 24) (EHdr Scratch24) ((EHdr Value)[48--24])  ;
+      {| st_op :=
+          extract(Scratch24) ;;
+          Value <- EConcat (m := 24) (EHdr Scratch24) ((EHdr (sz := sz) Value)[48--24])  ;
         st_trans := transition accept
       |}
     | ParseValue4 =>
-      {| st_op := 
-          extract(Scratch32) ;; 
-          Value <- EConcat (m := 16) (EHdr Scratch32) ((EHdr Value)[48--32])  ;
+      {| st_op :=
+          extract(Scratch32) ;;
+          Value <- EConcat (m := 16) (EHdr Scratch32) ((EHdr (sz := sz) Value)[48--32])  ;
         st_trans := transition accept
       |}
     | ParseValue5 =>
-      {| st_op := 
-          extract(Scratch40) ;; 
-          Value <- EConcat (m := 8) (EHdr Scratch40) ((EHdr Value)[48--40])  ;
+      {| st_op :=
+          extract(Scratch40) ;;
+          Value <- EConcat (m := 8) (EHdr Scratch40) ((EHdr (sz := sz) Value)[48--40])  ;
         st_trans := transition accept
       |}
     | ParseValue6 =>
@@ -205,9 +116,9 @@ Module TimestampRefKeepSingle.
       |}
     end.
 
-  Program Definition aut: Syntax.t state header :=
+  Program Definition aut: Syntax.t state sz :=
     {| t_states := states |}.
-  Solve Obligations with (destruct s; cbv; Lia.lia).
+  Solve Obligations with (destruct s || destruct h; cbv; Lia.lia).
 
 End TimestampRefKeepSingle.
 
@@ -222,134 +133,45 @@ Module TimestampRefZeroSingle.
   | ParseValue6.
 
   Scheme Equality for state.
-
   Global Instance state_eqdec: EquivDec.EqDec state eq := state_eq_dec.
-  Global Program Instance state_finite: @Finite state _ state_eq_dec :=
-    {| enum := [Start; ParseValue1; ParseValue2; ParseValue3; ParseValue4; ParseValue5; ParseValue6] |}.
-  Next Obligation.
-    repeat constructor;
-      repeat match goal with
-            | H: List.In _ [] |- _ => apply List.in_nil in H; exfalso; exact H
-            | |- ~ List.In _ [] => apply List.in_nil
-            | |- ~ List.In _ (_ :: _) => unfold not; intros
-            | H: List.In _ (_::_) |- _ => inversion H; clear H
-            | _ => discriminate
-            end.
-  Qed.
-  Next Obligation.
-    destruct x; intuition congruence.
-  Qed.
-
-  Inductive header : nat -> Type :=
-  | Typ : header 8
-  | Len : header 8
-  | Value : header 48
-  | Scratch8 : header 8
-  | Scratch16 : header 16
-  | Scratch24 : header 24
-  | Scratch32 : header 32
-  | Scratch40 : header 40.
-
-  Derive Signature for header.
-
-  Definition h16_eq_dec (x y: header 16) : {x = y} + {x <> y} :=
-    match x, y with 
-    | Scratch16, Scratch16 => left eq_refl
-    | _, _ => idProp
-    end.
-
-  Definition h24_eq_dec (x y: header 24) : {x = y} + {x <> y} :=
-    match x, y with 
-    | Scratch24, Scratch24 => left eq_refl
-    | _, _ => idProp
-    end.
-
-  Definition h32_eq_dec (x y: header 32) : {x = y} + {x <> y} :=
-    match x, y with 
-    | Scratch32, Scratch32 => left eq_refl
-    | _, _ => idProp
-    end.
-
-  Definition h40_eq_dec (x y: header 40) : {x = y} + {x <> y} :=
-    match x, y with 
-    | Scratch40, Scratch40 => left eq_refl
-    | _, _ => idProp
-    end.
-
-  Definition h48_eq_dec (x y: header 48) : {x = y} + {x <> y} :=
-    match x, y with 
-    | Value, Value => left eq_refl
-    | _, _ => idProp
-    end.
-
-  Definition h8_eq_dec (x y: header 8) : {x = y} + {x <> y}. 
-  refine (
-    match x with 
-    | Typ => 
-      match y with 
-      | Typ => left eq_refl
-      | Len => right _
-      | Scratch8 => right _
-      end
-    | Len => 
-      match y with 
-      | Typ => right _
-      | Len => left eq_refl
-      | Scratch8 => right _
-      end
-    | Scratch8 => 
-        match y with 
-        | Typ => right _
-        | Len => right _
-        | Scratch8 => left eq_refl
-        end
-    end
-  ); unfold "<>"; intros H; inversion H.
+  Global Instance state_finite: @Finite state _ state_eq_dec.
+  Proof.
+    solve_finiteness.
   Defined.
 
+  Inductive header :=
+  | Typ
+  | Len
+  | Value
+  | Scratch8
+  | Scratch16
+  | Scratch24
+  | Scratch32
+  | Scratch40.
 
-  Definition header_eqdec_ (n: nat) (x: header n) (y: header n) : {x = y} + {x <> y}.
-    solve_header_eqdec_ n x y 
-      ((existT (fun n => forall x y: header n, {x = y} + {x <> y}) _ h8_eq_dec) :: 
-        (existT _ _ h16_eq_dec) :: (existT _ _ h24_eq_dec) :: (existT _ _ h32_eq_dec) :: 
-        (existT _ _ h40_eq_dec) :: (existT _ _ h48_eq_dec) :: nil).
-  Defined. 
-
-  Global Instance header_eqdec: forall n, EquivDec.EqDec (header n) eq := header_eqdec_.
-
-  Global Instance header_eqdec': EquivDec.EqDec (Syntax.H' header) eq.
+  Scheme Equality for header.
+  Global Instance header_eqdec: EquivDec.EqDec header eq := header_eq_dec.
+  Global Instance header_finite: @Finite header _ header_eq_dec.
   Proof.
-    solve_eqdec'.
+    solve_finiteness.
   Defined.
 
-  Global Instance header_finite: forall n, @Finite (header n) _ _.
-  Proof.
-    intros n; solve_indexed_finiteness n [8; 16; 24; 32; 40; 48].
-  Qed.
-
-  Global Program Instance header_finite': @Finite {n & header n} _ header_eqdec' :=
-    {| enum := [ 
-      existT _ _ Len; existT _ _ Typ; existT _ _ Value;  
-      existT _ _ Scratch8; existT _ _ Scratch16; existT _ _ Scratch24;
-      existT _ _ Scratch32; existT _ _ Scratch40
-      
-      ] |}.
-  Next Obligation.
-    solve_header_finite.
-  Qed.
-  Next Obligation.
-  dependent destruction X; subst;
-  repeat (
-    match goal with
-    | |- ?L \/ ?R => (now left; trivial) || right
-    end
-  ).
-  Qed.
+  Definition sz (h: header): nat :=
+    match h with
+    | Typ => 8
+    | Len => 8
+    | Value => 48
+    | Scratch8 => 8
+    | Scratch16 => 16
+    | Scratch24 => 24
+    | Scratch32 => 32
+    | Scratch40 => 40
+    end.
 
   Definition states (s: state) :=
     match s with
     | Start =>
-      {| st_op := 
+      {| st_op :=
           extract(Typ) ;;
           extract(Len) ;
         st_trans := transition select (| EHdr Len |) {{
@@ -364,33 +186,33 @@ Module TimestampRefZeroSingle.
         }}
       |}
     | ParseValue1 =>
-      {| st_op := 
-          extract(Scratch8) ;; 
-          Value <- EConcat (n := 8) (EHdr Scratch8) (ELit (Ntuple.n_tuple_repeat 40 false))  ;
+      {| st_op :=
+          extract(Scratch8) ;;
+          Value <- EConcat (n := 8) (EHdr (sz := sz) Scratch8) (ELit _ (Ntuple.n_tuple_repeat 40 false))  ;
         st_trans := transition accept
       |}
     | ParseValue2 =>
-      {| st_op := 
-          extract(Scratch16) ;; 
-          Value <- EConcat (n := 16) (EHdr Scratch16) (ELit (Ntuple.n_tuple_repeat 32 false))  ;
+      {| st_op :=
+          extract(Scratch16) ;;
+          Value <- EConcat (n := 16) (EHdr (sz := sz) Scratch16) (ELit _ (Ntuple.n_tuple_repeat 32 false))  ;
         st_trans := transition accept
       |}
     | ParseValue3 =>
-      {| st_op := 
-          extract(Scratch24) ;; 
-          Value <- EConcat (n := 24) (EHdr Scratch24) (ELit (Ntuple.n_tuple_repeat 24 false))  ;
+      {| st_op :=
+          extract(Scratch24) ;;
+          Value <- EConcat (n := 24) (EHdr (sz := sz) Scratch24) (ELit _ (Ntuple.n_tuple_repeat 24 false))  ;
         st_trans := transition accept
       |}
     | ParseValue4 =>
-      {| st_op := 
-          extract(Scratch32) ;; 
-          Value <- EConcat (n := 32) (EHdr Scratch32) (ELit (Ntuple.n_tuple_repeat 16 false))  ;
+      {| st_op :=
+          extract(Scratch32) ;;
+          Value <- EConcat (n := 32) (EHdr (sz := sz) Scratch32) (ELit _ (Ntuple.n_tuple_repeat 16 false))  ;
         st_trans := transition accept
       |}
     | ParseValue5 =>
-      {| st_op := 
-          extract(Scratch40) ;; 
-          Value <- EConcat (n := 40) (EHdr Scratch40) (ELit (Ntuple.n_tuple_repeat 8 false))  ;
+      {| st_op :=
+          extract(Scratch40) ;;
+          Value <- EConcat (n := 40) (EHdr (sz := sz) Scratch40) (ELit _ (Ntuple.n_tuple_repeat 8 false))  ;
         st_trans := transition accept
       |}
     | ParseValue6 =>
@@ -399,9 +221,9 @@ Module TimestampRefZeroSingle.
       |}
     end.
 
-  Program Definition aut: Syntax.t state header :=
+  Program Definition aut: Syntax.t state sz :=
     {| t_states := states |}.
-  Solve Obligations with (destruct s; cbv; Lia.lia).
+  Solve Obligations with (destruct s || destruct h; cbv; Lia.lia).
 
 End TimestampRefZeroSingle.
 
@@ -417,165 +239,53 @@ Module TimestampSpecSingle.
   | ParseTimestamp.
 
   Scheme Equality for state.
-
   Global Instance state_eqdec: EquivDec.EqDec state eq := state_eq_dec.
-  Global Program Instance state_finite: @Finite state _ state_eq_dec :=
-    {| enum := [Start; ParseValue1; ParseValue2; ParseValue3; ParseValue4; ParseValue5; ParseValue6; ParseTimestamp] |}.
-  Next Obligation.
-    repeat constructor;
-      repeat match goal with
-            | H: List.In _ [] |- _ => apply List.in_nil in H; exfalso; exact H
-            | |- ~ List.In _ [] => apply List.in_nil
-            | |- ~ List.In _ (_ :: _) => unfold not; intros
-            | H: List.In _ (_::_) |- _ => inversion H; clear H
-            | _ => discriminate
-            end.
-  Qed.
-  Next Obligation.
-    destruct x; intuition congruence.
-  Qed.
-
-  Inductive header : nat -> Type :=
-  | Typ : header 8
-  | Len : header 8
-  | Scratch8 : header 8
-  | Scratch16 : header 16
-  | Scratch24 : header 24
-  | Scratch32 : header 32
-  | Scratch40 : header 40
-  | Scratch48 : header 48
-  | Pointer : header 8
-  | Overflow: header 4
-  | Flag: header 4
-  | Timestamp: header 32.
-
-  Derive Signature for header.
-
-  Definition h4_eq_dec (x y: header 4) : {x = y} + {x <> y}.
-  refine (
-    match x, y with
-    | Overflow, Flag => right _
-    | Flag, Overflow => right _ 
-    | Flag, Flag => left eq_refl
-    | Overflow, Overflow => left eq_refl
-    end
-  ); unfold "<>"; intros H; inversion H.
-  Defined.
-
-  Definition h16_eq_dec (x y: header 16) : {x = y} + {x <> y} :=
-    match x, y with 
-    | Scratch16, Scratch16 => left eq_refl
-    | _, _ => idProp
-    end.
-
-  Definition h24_eq_dec (x y: header 24) : {x = y} + {x <> y} :=
-    match x, y with 
-    | Scratch24, Scratch24 => left eq_refl
-    | _, _ => idProp
-    end.
-
-  Definition h32_eq_dec (x y: header 32) : {x = y} + {x <> y}.
-  refine (
-    match x, y with
-    | Scratch32, Timestamp => right _
-    | Timestamp, Scratch32 => right _ 
-    | Timestamp, Timestamp => left eq_refl
-    | Scratch32, Scratch32 => left eq_refl
-    end
-  ); unfold "<>"; intros H; inversion H.
-  Defined.
-
-
-  Definition h40_eq_dec (x y: header 40) : {x = y} + {x <> y} :=
-    match x, y with 
-    | Scratch40, Scratch40 => left eq_refl
-    | _, _ => idProp
-    end.
-
-  Definition h48_eq_dec (x y: header 48) : {x = y} + {x <> y} :=
-    match x, y with 
-    | Scratch48, Scratch48 => left eq_refl
-    | _, _ => idProp
-    end.
-
-  Definition h8_eq_dec (x y: header 8) : {x = y} + {x <> y}. 
-  refine (
-    match x with 
-    | Typ => 
-      match y with 
-      | Typ => left eq_refl
-      | Len => right _
-      | Scratch8 => right _
-      | Pointer => right _
-      end
-    | Len => 
-      match y with 
-      | Typ => right _
-      | Len => left eq_refl
-      | Scratch8 => right _
-      | Pointer => right _
-      end
-    | Scratch8 => 
-        match y with 
-        | Typ => right _
-        | Len => right _
-        | Scratch8 => left eq_refl
-        | Pointer => right _
-        end
-    | Pointer => 
-      match y with 
-      | Typ => right _
-      | Len => right _
-      | Scratch8 => right _
-      | Pointer => left eq_refl
-      end
-    end
-  ); unfold "<>"; intros H; inversion H.
-  Defined.
-
-
-  Definition header_eqdec_ (n: nat) (x: header n) (y: header n) : {x = y} + {x <> y}.
-    solve_header_eqdec_ n x y 
-      ((existT (fun n => forall x y: header n, {x = y} + {x <> y}) _ h8_eq_dec) :: 
-        (existT _ _ h16_eq_dec) :: (existT _ _ h24_eq_dec) :: (existT _ _ h32_eq_dec) :: 
-        (existT _ _ h40_eq_dec) :: (existT _ _ h48_eq_dec) :: (existT _ _ h4_eq_dec) :: nil).
-  Defined. 
-
-  Global Instance header_eqdec: forall n, EquivDec.EqDec (header n) eq := header_eqdec_.
-
-  Global Instance header_eqdec': EquivDec.EqDec (Syntax.H' header) eq.
+  Global Instance state_finite: @Finite state _ state_eq_dec.
   Proof.
-    solve_eqdec'.
+    solve_finiteness.
   Defined.
 
-  Global Instance header_finite: forall n, @Finite (header n) _ _.
+  Inductive header :=
+  | Typ
+  | Len
+  | Scratch8
+  | Scratch16
+  | Scratch24
+  | Scratch32
+  | Scratch40
+  | Scratch48
+  | Pointer
+  | Overflow
+  | Flag
+  | Timestamp.
+
+  Definition sz (h: header): nat :=
+    match h with
+    | Typ => 8
+    | Len => 8
+    | Scratch8 => 8
+    | Scratch16 => 16
+    | Scratch24 => 24
+    | Scratch32 => 32
+    | Scratch40 => 40
+    | Scratch48 => 48
+    | Pointer => 8
+    | Overflow => 4
+    | Flag => 4
+    | Timestamp => 32
+    end.
+
+  Scheme Equality for header.
+  Global Instance header_eqdec: EquivDec.EqDec header eq := header_eq_dec.
+  Global Instance header_finite: @Finite header _ header_eq_dec.
   Proof.
-    intros n; solve_indexed_finiteness n [4; 8; 16; 24; 32; 40; 48].
-  Qed.
+    solve_finiteness.
+  Defined.
 
-  Global Program Instance header_finite': @Finite {n & header n} _ header_eqdec' :=
-    {| enum := [ 
-      existT _ _ Len; existT _ _ Typ;
-      existT _ _ Scratch8; existT _ _ Scratch16; existT _ _ Scratch24;
-      existT _ _ Scratch32; existT _ _ Scratch40; existT _ _ Scratch48;
-      existT _ _ Overflow; existT _ _ Flag; existT _ _ Pointer; existT _ _ Timestamp
-      ] |}.
-  Next Obligation.
-    solve_header_finite.
-  Qed.
-  Next Obligation.
-  dependent destruction X; subst;
-  repeat (
-    match goal with
-    | |- ?L \/ ?R => (now left; trivial) || right
-    end
-  ).
-  Qed.
-
-  Definition states (s: state) :=
+  Definition states (s: state) : Syntax.state state sz :=
     match s with
     | Start =>
-      {| st_op := 
+      {| st_op :=
           extract(Typ) ;;
           extract(Len) ;
         st_trans := transition select (| EHdr Typ, EHdr Len |) {{
@@ -591,7 +301,7 @@ Module TimestampSpecSingle.
         }}
       |}
     | ParseTimestamp =>
-      {| st_op := 
+      {| st_op :=
           extract(Pointer) ;;
           extract(Overflow) ;;
           extract(Flag) ;;
@@ -599,27 +309,27 @@ Module TimestampSpecSingle.
         st_trans := transition accept (* TODO: validate pointer and flag? *)
       |}
     | ParseValue1 =>
-      {| st_op := 
+      {| st_op :=
           extract(Scratch8) ;
         st_trans := transition accept
       |}
     | ParseValue2 =>
-      {| st_op := 
+      {| st_op :=
           extract(Scratch16) ;
         st_trans := transition accept
       |}
     | ParseValue3 =>
-      {| st_op := 
+      {| st_op :=
           extract(Scratch24) ;
         st_trans := transition accept
       |}
     | ParseValue4 =>
-      {| st_op := 
+      {| st_op :=
           extract(Scratch32) ;
         st_trans := transition accept
       |}
     | ParseValue5 =>
-      {| st_op := 
+      {| st_op :=
           extract(Scratch40) ;
         st_trans := transition accept
       |}
@@ -629,9 +339,9 @@ Module TimestampSpecSingle.
       |}
     end.
 
-  Program Definition aut: Syntax.t state header :=
+  Program Definition aut: Syntax.t state sz :=
     {| t_states := states |}.
-  Solve Obligations with (destruct s; cbv; Lia.lia).
+  Solve Obligations with (destruct s || destruct h; cbv; Lia.lia).
 
 End TimestampSpecSingle.
 
@@ -644,92 +354,37 @@ Module TimestampRefSmall.
   | Parse3.
 
   Scheme Equality for state.
-
   Global Instance state_eqdec: EquivDec.EqDec state eq := state_eq_dec.
-  Global Program Instance state_finite: @Finite state _ state_eq_dec :=
-    {| enum := [Start; Parse1; Parse2; Parse3] |}.
-  Next Obligation.
-    repeat constructor;
-      repeat match goal with
-             | H: List.In _ [] |- _ => apply List.in_nil in H; exfalso; exact H
-             | |- ~ List.In _ [] => apply List.in_nil
-             | |- ~ List.In _ (_ :: _) => unfold not; intros
-             | H: List.In _ (_::_) |- _ => inversion H; clear H
-             | _ => discriminate
-             end.
-  Qed.
-  Next Obligation.
-    destruct x; intuition congruence.
-  Qed.
-
-  Inductive header : nat -> Type :=
-  | Len : header 2
-  | Pref1 : header 8
-  | Pref2: header 16
-  | Timestamps : header 24.
-
-  Derive Signature for header.
-
-  Definition h2_eq_dec (x y: header 2) : {x = y} + {x <> y} :=
-    match x, y with 
-    | Len, Len => left eq_refl
-    | _, _ => idProp
-    end.
-
-  Definition h8_eq_dec (x y: header 8) : {x = y} + {x <> y} :=
-    match x, y with 
-    | Pref1, Pref1 => left eq_refl
-    | _, _ => idProp
-    end.
-
-  Definition h16_eq_dec (x y: header 16) : {x = y} + {x <> y} :=
-    match x, y with 
-    | Pref2, Pref2 => left eq_refl
-    | _, _ => idProp
-    end.
-
-  Definition h24_eq_dec (x y: header 24) : {x = y} + {x <> y} :=
-    match x, y with 
-    | Timestamps, Timestamps => left eq_refl
-    | _, _ => idProp
-    end.
-
-  Definition header_eqdec_ (n: nat) (x: header n) (y: header n) : {x = y} + {x <> y}.
-    solve_header_eqdec_ n x y 
-      ((existT (fun n => forall x y: header n, {x = y} + {x <> y}) 2 h2_eq_dec) :: 
-        (existT _ 8 h8_eq_dec) :: (existT _ 16 h16_eq_dec) :: (existT _ 24 h24_eq_dec) :: nil).
-  Defined. 
-
-  Global Instance header_eqdec: forall n, EquivDec.EqDec (header n) eq := header_eqdec_.
-
-  Global Instance header_eqdec': EquivDec.EqDec (Syntax.H' header) eq.
+  Global Instance state_finite: @Finite state _ state_eq_dec.
   Proof.
-    solve_eqdec'.
+    solve_finiteness.
   Defined.
 
-  Global Instance header_finite: forall n, @Finite (header n) _ _.
-  Proof.
-    intros n; solve_indexed_finiteness n [24; 16; 8; 2].
-  Qed.
+  Inductive header :=
+  | Len
+  | Pref1
+  | Pref2
+  | Timestamps.
 
-  Global Program Instance header_finite': @Finite {n & header n} _ header_eqdec' :=
-    {| enum := [ existT _ _ Len; existT _ _ Pref1; existT _ _ Pref2;  existT _ _ Timestamps] |}.
-  Next Obligation.
-    solve_header_finite.
-  Qed.
-  Next Obligation.
-  dependent destruction X; subst;
-  repeat (
-    match goal with
-    | |- ?L \/ ?R => (now left; trivial) || right
-    end
-  ).
-  Qed.
+  Definition sz (h: header): nat :=
+    match h with
+    | Len => 2
+    | Pref1 => 8
+    | Pref2 => 16
+    | Timestamps => 24
+    end.
+
+  Scheme Equality for header.
+  Global Instance header_eqdec: EquivDec.EqDec header eq := header_eq_dec.
+  Global Instance header_finite: @Finite header _ header_eq_dec.
+  Proof.
+    solve_finiteness.
+  Defined.
 
   Definition states (s: state) :=
     match s with
     | Start =>
-      {| st_op := 
+      {| st_op :=
           extract(Len) ;
          st_trans := transition select (| EHdr Len |) {{
            [| exact #b|0|0 |] ==> accept ;;;
@@ -740,15 +395,15 @@ Module TimestampRefSmall.
          }}
       |}
     | Parse1 =>
-      {| st_op := 
-          extract(Pref1) ;; 
-          Timestamps <- EConcat (m := 16) (EHdr Pref1) ((EHdr Timestamps)[24--8])  ;
+      {| st_op :=
+          extract(Pref1) ;;
+          Timestamps <- EConcat (m := 16) (EHdr Pref1) ((EHdr (sz := sz) Timestamps)[24--8])  ;
          st_trans := transition accept
       |}
     | Parse2 =>
-      {| st_op := 
-          extract(Pref2) ;; 
-          Timestamps <- EConcat (m := 8) (EHdr Pref2) ((EHdr Timestamps)[24--16]) ;
+      {| st_op :=
+          extract(Pref2) ;;
+          Timestamps <- EConcat (m := 8) (EHdr Pref2) ((EHdr (sz := sz) Timestamps)[24--16]) ;
          st_trans := transition accept
       |}
     | Parse3 =>
@@ -757,12 +412,11 @@ Module TimestampRefSmall.
       |}
     end.
 
-  Program Definition aut: Syntax.t state header :=
+  Program Definition aut: Syntax.t state sz :=
     {| t_states := states |}.
-  Solve Obligations with (destruct s; cbv; Lia.lia).
+  Solve Obligations with (destruct s || destruct h; cbv; Lia.lia).
 
 End TimestampRefSmall.
-
 
 Module TimestampSpecSmall.
   Inductive state :=
@@ -772,99 +426,35 @@ Module TimestampSpecSmall.
   | Parse3.
 
   Scheme Equality for state.
-
   Global Instance state_eqdec: EquivDec.EqDec state eq := state_eq_dec.
-  Global Program Instance state_finite: @Finite state _ state_eq_dec :=
-    {| enum := [Start; Parse1; Parse2; Parse3] |}.
-  Next Obligation.
-    repeat constructor;
-      repeat match goal with
-             | H: List.In _ [] |- _ => apply List.in_nil in H; exfalso; exact H
-             | |- ~ List.In _ [] => apply List.in_nil
-             | |- ~ List.In _ (_ :: _) => unfold not; intros
-             | H: List.In _ (_::_) |- _ => inversion H; clear H
-             | _ => discriminate
-             end.
-  Qed.
-  Next Obligation.
-    destruct x; intuition congruence.
-  Qed.
+  Global Instance state_finite: @Finite state _ state_eq_dec.
+  Proof.
+    solve_finiteness.
+  Defined.
 
-  Inductive header : nat -> Type :=
-  | Len : header 2
-  | T1 : header 8
-  | T2 : header 8 
-  | T3 : header 8.
+  Inductive header :=
+  | Len
+  | T1
+  | T2
+  | T3.
 
-  Derive Signature for header.
-
-  Definition h2_eq_dec (x y: header 2) : {x = y} + {x <> y} :=
-    match x, y with 
-    | Len, Len => left eq_refl
-    | _, _ => idProp
+  Definition sz (h: header): nat :=
+    match h with
+    | Len => 2
+    | T1 | T2 | T3 => 8
     end.
 
-  Definition h8_eq_dec (x y: header 8) : {x = y} + {x <> y}.
-  refine (
-    match x with 
-    | T1 => 
-      match y with 
-      | T1 => left eq_refl
-      | T2 => right _
-      | T3 => right _
-      end
-    | T2 => 
-      match y with 
-      | T1 => right _
-      | T2 => left eq_refl
-      | T3 => right _
-      end
-    | T3 => 
-      match y with 
-      | T1 => right _
-      | T2 => right _
-      | T3 => left eq_refl
-      end
-    end
-  ); intros H; inversion H.
+  Scheme Equality for header.
+  Global Instance header_eqdec: EquivDec.EqDec header eq := header_eq_dec.
+  Global Instance header_finite: @Finite header _ header_eq_dec.
+  Proof.
+    solve_finiteness.
   Defined.
 
-  Definition header_eqdec_ (n: nat) (x: header n) (y: header n) : {x = y} + {x <> y}.
-    solve_header_eqdec_ n x y 
-      ((existT (fun n => forall x y: header n, {x = y} + {x <> y}) 2 h2_eq_dec) :: 
-        (existT _ 8 h8_eq_dec) :: nil).
-  Defined. 
-
-  Global Instance header_eqdec: forall n, EquivDec.EqDec (header n) eq := header_eqdec_.
-
-  Global Instance header_eqdec': EquivDec.EqDec (Syntax.H' header) eq.
-  Proof.
-    solve_eqdec'.
-  Defined.
-
-  Global Instance header_finite: forall n, @Finite (header n) _ _.
-  Proof.
-    intros n; solve_indexed_finiteness n [8; 2].
-  Qed.
-
-  Global Program Instance header_finite': @Finite {n & header n} _ header_eqdec' :=
-    {| enum := [ existT _ _ Len; existT _ _ T1; existT _ _ T2;  existT _ _ T3] |}.
-  Next Obligation.
-    solve_header_finite.
-  Qed.
-  Next Obligation.
-  dependent destruction X; subst;
-  repeat (
-    match goal with
-    | |- ?L \/ ?R => (now left; trivial) || right
-    end
-  ).
-  Qed.
-
-  Definition states (s: state) :=
+  Definition states (s: state) : Syntax.state state sz :=
     match s with
     | Start =>
-      {| st_op := 
+      {| st_op :=
           extract(Len) ;
          st_trans := transition select (| EHdr Len |) {{
            [| exact #b|0|0 |] ==> accept ;;;
@@ -875,31 +465,30 @@ Module TimestampSpecSmall.
          }}
       |}
     | Parse1 =>
-      {| st_op := 
+      {| st_op :=
           extract(T1) ;
          st_trans := transition accept
       |}
     | Parse2 =>
-      {| st_op := 
-          extract(T1) ;; 
+      {| st_op :=
+          extract(T1) ;;
           extract(T2) ;
          st_trans := transition accept
       |}
     | Parse3 =>
-      {| st_op := 
-          extract(T1) ;; 
-          extract(T2) ;; 
+      {| st_op :=
+          extract(T1) ;;
+          extract(T2) ;;
           extract(T3) ;
          st_trans := transition accept
       |}
     end.
 
-  Program Definition aut: Syntax.t state header :=
+  Program Definition aut: Syntax.t state sz :=
     {| t_states := states |}.
-  Solve Obligations with (destruct s; cbv; Lia.lia).
+  Solve Obligations with (destruct s || destruct h; cbv; Lia.lia).
 
 End TimestampSpecSmall.
-
 
 (* parse 2 options of between 0-6 bytes, and if a timestamp option is present, parse it into a timestamp structure *)
 Module TimestampSpec2.
@@ -912,7 +501,7 @@ Module TimestampSpec2.
 
   | Parse01
   | Parse11
-  
+
   | Parse02
   | Parse12
 
@@ -929,221 +518,62 @@ Module TimestampSpec2.
   | Parse16.
 
   Scheme Equality for state.
-
   Global Instance state_eqdec: EquivDec.EqDec state eq := state_eq_dec.
-  Global Program Instance state_finite: @Finite state _ state_eq_dec :=
-    {| enum := [  Parse0 ; Parse1; 
-    Parse0S ; Parse1S;
-    Parse01 ; Parse11;
-    Parse02 ; Parse12;
-    Parse03 ; Parse13;
-    Parse04 ; Parse14;
-    Parse05 ; Parse15;
-    Parse06 ; Parse16 ]; |}.
-  Next Obligation.
-    repeat constructor;
-      repeat match goal with
-             | H: List.In _ [] |- _ => apply List.in_nil in H; exfalso; exact H
-             | |- ~ List.In _ [] => apply List.in_nil
-             | |- ~ List.In _ (_ :: _) => unfold not; intros
-             | H: List.In _ (_::_) |- _ => inversion H; clear H
-             | _ => discriminate
-             end.
-  Qed.
-  Next Obligation.
-    destruct x; intuition congruence.
-  Qed.
-
-  Inductive header : nat -> Type :=
-  | Scratch8 : header 8
-  | Scratch16 : header 16
-  | Scratch24 : header 24
-  | Scratch32 : header 32
-  | Scratch40 : header 40
-  | T0 : header 8
-  | L0 : header 8
-  | V0 : header 48
-  | T1 : header 8
-  | L1 : header 8
-  | V1 : header 48
-  | Pointer : header 8
-  | Overflow: header 4
-  | Flag: header 4
-  | Timestamp: header 32.
-
-  Derive Signature for header.
-
-  Definition h4_eq_dec (x y: header 4) : {x = y} + {x <> y}.
-  refine (
-    match x, y with
-    | Overflow, Flag => right _
-    | Flag, Overflow => right _
-    | Overflow, Overflow => left eq_refl
-    | Flag, Flag => left eq_refl
-    end
-  ); intros H; inversion H.
-  Defined.
-
-  Definition h8_eq_dec (x y: header 8) : {x = y} + {x <> y}.
-  refine (
-    match x with 
-    | Scratch8 =>
-      match y with
-      | Scratch8  => left eq_refl
-      | T0 => right _
-      | L0 => right _
-      | T1 => right _
-      | L1 => right _
-      | Pointer => right _
-      end
-    | T0 =>
-      match y with
-      | Scratch8  => right _
-      | T0 => left eq_refl
-      | L0 => right _
-      | T1 => right _
-      | L1 => right _
-      | Pointer => right _
-      end
-      
-    | L0 =>
-      match y with
-      | Scratch8  => right _
-      | T0 => right _
-      | L0 => left eq_refl
-      | T1 => right _
-      | L1 => right _
-      | Pointer => right _
-      end
-      
-    | T1 =>
-      match y with
-      | Scratch8  => right _
-      | T0 => right _
-      | L0 => right _
-      | T1 => left eq_refl
-      | L1 => right _
-      | Pointer => right _
-      end
-      
-    | L1 =>
-      match y with
-      | Scratch8  => right _
-      | T0 => right _
-      | L0 => right _
-      | T1 => right _
-      | L1 => left eq_refl
-      | Pointer => right _
-      end
-    | Pointer => 
-      match y with
-      | Scratch8  => right _
-      | T0 => right _
-      | L0 => right _
-      | T1 => right _
-      | L1 => right _
-      | Pointer => left eq_refl
-      end
-    end
-  ); intros H; inversion H.
-  Defined.
-
-  Definition h16_eq_dec (x y: header 16) : {x = y} + {x <> y} :=
-    match x, y with 
-    | Scratch16, Scratch16 => left eq_refl
-    end.
-  Definition h24_eq_dec (x y: header 24) : {x = y} + {x <> y} :=
-    match x, y with 
-    | Scratch24, Scratch24 => left eq_refl
-    end.
-  Definition h32_eq_dec (x y: header 32) : {x = y} + {x <> y}.
-  refine (
-    match x, y with 
-    | Scratch32, Scratch32 => left eq_refl
-    | Timestamp, Timestamp => left eq_refl
-    | Timestamp, Scratch32 => right _
-    | Scratch32, Timestamp => right _
-    end
-  ); intros H; inversion H.
-  Defined.
-
-  Definition h40_eq_dec (x y: header 40) : {x = y} + {x <> y} :=
-    match x, y with 
-    | Scratch40, Scratch40 => left eq_refl
-    end.
-
-  Definition h48_eq_dec (x y: header 48) : {x = y} + {x <> y}.
-    refine (
-    match x with 
-    | V0 =>
-      match y with
-      | V0 => left eq_refl
-      | V1 => right _
-      end
-    | V1 =>
-      match y with
-      | V0 => right _
-      | V1 => left eq_refl
-      end
-    end
-  ); intros H; inversion H.
-  Defined.
-
-  Definition header_eqdec_ (n: nat) (x: header n) (y: header n) : {x = y} + {x <> y}.
-    solve_header_eqdec_ n x y 
-      ((existT (fun n => forall x y: header n, {x = y} + {x <> y}) _ h8_eq_dec) :: 
-        (existT _ _ h16_eq_dec) :: (existT _ _ h24_eq_dec) :: (existT _ _ h32_eq_dec) :: 
-        (existT _ _ h40_eq_dec) :: (existT _ _ h48_eq_dec) :: (existT _ _ h4_eq_dec) :: nil).
-  Defined. 
-
-  Global Instance header_eqdec: forall n, EquivDec.EqDec (header n) eq := header_eqdec_.
-
-  Global Instance header_eqdec': EquivDec.EqDec (Syntax.H' header) eq.
+  Global Instance state_finite: @Finite state _ state_eq_dec.
   Proof.
-    solve_eqdec'.
+    solve_finiteness.
   Defined.
 
-  Global Instance header_finite: forall n, @Finite (header n) _ _.
+  Inductive header :=
+  | Scratch8
+  | Scratch16
+  | Scratch24
+  | Scratch32
+  | Scratch40
+  | T0
+  | L0
+  | V0
+  | T1
+  | L1
+  | V1
+  | Pointer
+  | Overflow
+  | Flag
+  | Timestamp.
+
+  Definition sz (h: header): nat :=
+    match h with
+    | Scratch8  => 8
+    | Scratch16  => 16
+    | Scratch24  => 24
+    | Scratch32  => 32
+    | Scratch40  => 40
+    | T0  => 8
+    | L0  => 8
+    | V0  => 48
+    | T1  => 8
+    | L1  => 8
+    | V1  => 48
+    | Pointer  => 8
+    | Overflow => 4
+    | Flag => 4
+    | Timestamp => 32
+    end.
+
+  Scheme Equality for header.
+  Global Instance header_eqdec: EquivDec.EqDec header eq := header_eq_dec.
+  Global Instance header_finite: @Finite header _ header_eq_dec.
   Proof.
-    intros n; solve_indexed_finiteness n [4; 8; 16; 24; 32; 40; 48].
-  Qed.
+    solve_finiteness.
+  Defined.
 
-  Global Program Instance header_finite': @Finite {n & header n} _ header_eqdec' :=
-    {| enum :=   [existT _ _ Scratch8 ;
-    existT _ _ Scratch16 ;
-    existT _ _ Scratch24 ;
-    existT _ _ Scratch32 ;
-    existT _ _ Scratch40 ;
-    existT _ _ T0 ;
-    existT _ _ L0 ;
-    existT _ _ V0 ;
-    existT _ _ T1 ;
-    existT _ _ L1 ;
-    existT _ _ V1 ;
-    existT _ _ Timestamp ;
-    existT _ _ Pointer ;
-    existT _ _ Overflow ;
-    existT _ _ Flag 
-    ]; |}.
-  Next Obligation.
-    solve_header_finite.
-  Qed.
-  Next Obligation.
-  dependent destruction X; subst;
-  repeat (
-    match goal with
-    | |- ?L \/ ?R => (now left; trivial) || right
-    end
-  ).
-  Qed.
-
-  Definition states (s: state) :=
+  Definition states (s: state) : Syntax.state state sz :=
     match s with
     | Parse0 =>
-      {| st_op := 
+      {| st_op :=
           extract(T0) ;;
           extract(L0) ;
-         st_trans := transition select (| EHdr T0, EHdr L0 |) {{
+         st_trans := transition select (| EHdr (sz := sz) T0, EHdr (sz := sz) L0 |) {{
            [| exact #b|0|1|0|0|0|1|0|0, exact #b|0|0|0|0|0|1|1|0 |] ==> inl Parse0S;;;
            [| exact #b|0|0|0|0|0|0|0|0, exact #b|0|0|0|0|0|0|0|0 |] ==> accept ;;;
            [| exact #b|0|0|0|0|0|0|0|1, exact #b|0|0|0|0|0|0|0|0 |] ==> accept ;;;
@@ -1157,43 +587,43 @@ Module TimestampSpec2.
          }}
       |}
     | Parse01 =>
-      {| st_op := 
+      {| st_op :=
           extract(Scratch8) ;;
-          V0 <- EConcat (m := 40) (EHdr Scratch8) ((EHdr V0)[48--8]) ;
+          V0 <- EConcat (m := 40) (EHdr (sz := sz) Scratch8) ((EHdr (sz := sz) V0)[48--8]) ;
          st_trans := transition inl Parse1;
       |}
     | Parse02 =>
-      {| st_op := 
+      {| st_op :=
           extract(Scratch16) ;;
-          V0 <- EConcat (m := 32) (EHdr Scratch16) ((EHdr V0)[48--16]) ;
+          V0 <- EConcat (m := 32) (EHdr (sz := sz) Scratch16) ((EHdr (sz := sz) V0)[48--16]) ;
          st_trans := transition inl Parse1;
       |}
     | Parse03 =>
-      {| st_op := 
+      {| st_op :=
           extract(Scratch24) ;;
-          V0 <- EConcat (m := 24) (EHdr Scratch24) ((EHdr V0)[48--24]) ;
+          V0 <- EConcat (m := 24) (EHdr (sz := sz) Scratch24) ((EHdr (sz := sz) V0)[48--24]) ;
          st_trans := transition inl Parse1;
       |}
     | Parse04 =>
-      {| st_op := 
+      {| st_op :=
           extract(Scratch32) ;;
-          V0 <- EConcat (m := 16) (EHdr Scratch32) ((EHdr V0)[48--32]) ;
+          V0 <- EConcat (m := 16) (EHdr (sz := sz) Scratch32) ((EHdr (sz := sz) V0)[48--32]) ;
          st_trans := transition inl Parse1;
       |}
     | Parse05 =>
-      {| st_op := 
+      {| st_op :=
           extract(Scratch40) ;;
-          V0 <- EConcat (m := 8) (EHdr Scratch40) ((EHdr V0)[48--40]) ;
+          V0 <- EConcat (m := 8) (EHdr (sz := sz) Scratch40) ((EHdr (sz := sz) V0)[48--40]) ;
          st_trans := transition inl Parse1;
       |}
     | Parse06 =>
-      {| st_op := 
+      {| st_op :=
           extract(V0) ;
          st_trans := transition inl Parse1;
       |}
 
     | Parse0S =>
-      {| st_op := 
+      {| st_op :=
           extract(Pointer) ;;
           extract(Overflow) ;;
           extract(Flag) ;;
@@ -1202,10 +632,10 @@ Module TimestampSpec2.
       |}
 
     | Parse1 =>
-      {| st_op := 
+      {| st_op :=
           extract(T1) ;;
           extract(L1) ;
-         st_trans := transition select (| EHdr T1, EHdr L1 |) {{
+         st_trans := transition select (| EHdr (sz := sz) T1, EHdr (sz := sz) L1 |) {{
            [| exact #b|0|1|0|0|0|1|0|0, exact #b|0|0|0|0|0|1|1|0 |] ==> inl Parse1S;;;
            [| exact #b|0|0|0|0|0|0|0|0, exact #b|0|0|0|0|0|0|0|0 |] ==> accept ;;;
            [| exact #b|0|0|0|0|0|0|0|1, exact #b|0|0|0|0|0|0|0|0 |] ==> accept ;;;
@@ -1219,42 +649,42 @@ Module TimestampSpec2.
          }}
       |}
     | Parse11 =>
-      {| st_op := 
+      {| st_op :=
           extract(Scratch8) ;;
-          V1 <- EConcat (m := 40) (EHdr Scratch8) ((EHdr V1)[48--8]) ;
+          V1 <- EConcat (m := 40) (EHdr (sz := sz) Scratch8) ((EHdr (sz := sz) V1)[48--8]) ;
          st_trans := transition accept;
       |}
     | Parse12 =>
-      {| st_op := 
+      {| st_op :=
           extract(Scratch16) ;;
-          V1 <- EConcat (m := 32) (EHdr Scratch16) ((EHdr V1)[48--16]) ;
+          V1 <- EConcat (m := 32) (EHdr (sz := sz) Scratch16) ((EHdr (sz := sz) V1)[48--16]) ;
          st_trans := transition accept;
       |}
     | Parse13 =>
-      {| st_op := 
+      {| st_op :=
           extract(Scratch24) ;;
-          V1 <- EConcat (m := 24) (EHdr Scratch24) ((EHdr V1)[48--24]) ;
+          V1 <- EConcat (m := 24) (EHdr (sz := sz) Scratch24) ((EHdr (sz := sz) V1)[48--24]) ;
          st_trans := transition accept;
       |}
     | Parse14 =>
-      {| st_op := 
+      {| st_op :=
           extract(Scratch32) ;;
-          V1 <- EConcat (m := 16) (EHdr Scratch32) ((EHdr V1)[48--32]) ;
+          V1 <- EConcat (m := 16) (EHdr (sz := sz) Scratch32) ((EHdr (sz := sz) V1)[48--32]) ;
          st_trans := transition accept;
       |}
     | Parse15 =>
-      {| st_op := 
+      {| st_op :=
           extract(Scratch40) ;;
-          V1 <- EConcat (m := 8) (EHdr Scratch40) ((EHdr V1)[48--40]) ;
+          V1 <- EConcat (m := 8) (EHdr (sz := sz) Scratch40) ((EHdr (sz := sz) V1)[48--40]) ;
          st_trans := transition accept;
       |}
     | Parse16 =>
-      {| st_op := 
+      {| st_op :=
           extract(V1) ;
          st_trans := transition accept;
       |}
     | Parse1S =>
-      {| st_op := 
+      {| st_op :=
           extract(Pointer) ;;
           extract(Overflow) ;;
           extract(Flag) ;;
@@ -1263,12 +693,11 @@ Module TimestampSpec2.
       |}
     end.
 
-  Program Definition aut: Syntax.t state header :=
+  Program Definition aut: Syntax.t state sz :=
     {| t_states := states |}.
-  Solve Obligations with (destruct s; cbv; Lia.lia).
+  Solve Obligations with (destruct s || destruct h; cbv; Lia.lia).
 
 End TimestampSpec2.
-
 
 
 (* parse 3 options of between 0-6 bytes, and if a timestamp option is present, parse it into a timestamp structure *)
@@ -1285,7 +714,7 @@ Module TimestampSpec3.
   | Parse01
   | Parse11
   | Parse21
-  
+
   | Parse02
   | Parse12
   | Parse22
@@ -1307,272 +736,68 @@ Module TimestampSpec3.
   | Parse26.
 
   Scheme Equality for state.
-
   Global Instance state_eqdec: EquivDec.EqDec state eq := state_eq_dec.
-  Global Program Instance state_finite: @Finite state _ state_eq_dec :=
-    {| enum := [  Parse0 ; Parse1; Parse2; 
-    Parse0S ; Parse1S; Parse2S
-    ; Parse01 ; Parse11; Parse21
-      ; Parse02 ; Parse12; Parse22
-    ; Parse03 ; Parse13; Parse23
-    ; Parse04 ; Parse14; Parse24
-    ; Parse05 ; Parse15; Parse25
-    ; Parse06 ; Parse16; Parse26 ]; |}.
-  Next Obligation.
-    repeat constructor;
-      repeat match goal with
-             | H: List.In _ [] |- _ => apply List.in_nil in H; exfalso; exact H
-             | |- ~ List.In _ [] => apply List.in_nil
-             | |- ~ List.In _ (_ :: _) => unfold not; intros
-             | H: List.In _ (_::_) |- _ => inversion H; clear H
-             | _ => discriminate
-             end.
-  Qed.
-  Next Obligation.
-    destruct x; intuition congruence.
-  Qed.
-
-  Inductive header : nat -> Type :=
-  | Scratch8 : header 8
-  | Scratch16 : header 16
-  | Scratch24 : header 24
-  | Scratch32 : header 32
-  | Scratch40 : header 40
-  | T0 : header 8
-  | L0 : header 8
-  | V0 : header 48
-  | T1 : header 8
-  | L1 : header 8
-  | V1 : header 48
-  | T2 : header 8
-  | L2 : header 8
-  | V2 : header 48
-  | Pointer : header 8
-  | Overflow: header 4
-  | Flag: header 4
-  | Timestamp: header 32.
-
-  Derive Signature for header.
-
-  Definition h4_eq_dec (x y: header 4) : {x = y} + {x <> y}.
-  refine (
-    match x, y with
-    | Overflow, Flag => right _
-    | Flag, Overflow => right _
-    | Overflow, Overflow => left eq_refl
-    | Flag, Flag => left eq_refl
-    end
-  ); intros H; inversion H.
-  Defined.
-
-  Definition h8_eq_dec (x y: header 8) : {x = y} + {x <> y}.
-  refine (
-    match x with 
-    | Scratch8 =>
-      match y with
-      | Scratch8  => left eq_refl
-      | T0 => right _
-      | L0 => right _
-      | T1 => right _
-      | L1 => right _
-      | T2 => right _
-      | L2 => right _
-      | Pointer => right _
-      end
-    | T0 =>
-      match y with
-      | Scratch8  => right _
-      | T0 => left eq_refl
-      | L0 => right _
-      | T1 => right _
-      | L1 => right _
-      | T2 => right _
-      | L2 => right _
-      | Pointer => right _
-      end
-      
-    | L0 =>
-      match y with
-      | Scratch8  => right _
-      | T0 => right _
-      | L0 => left eq_refl
-      | T1 => right _
-      | L1 => right _
-      | T2 => right _
-      | L2 => right _
-      | Pointer => right _
-      end
-      
-    | T1 =>
-      match y with
-      | Scratch8  => right _
-      | T0 => right _
-      | L0 => right _
-      | T1 => left eq_refl
-      | L1 => right _
-      | T2 => right _
-      | L2 => right _
-      | Pointer => right _
-      end
-      
-    | L1 =>
-      match y with
-      | Scratch8  => right _
-      | T0 => right _
-      | L0 => right _
-      | T1 => right _
-      | L1 => left eq_refl
-      | T2 => right _
-      | L2 => right _
-      | Pointer => right _
-      end
-    | T2 => 
-      match y with
-      | Scratch8  => right _
-      | T0 => right _
-      | L0 => right _
-      | T1 => right _
-      | L1 => right _
-      | T2 => left eq_refl
-      | L2 => right _
-      | Pointer => right _
-      end
-    | L2 => 
-      match y with
-      | Scratch8  => right _
-      | T0 => right _
-      | L0 => right _
-      | T1 => right _
-      | L1 => right _
-      | T2 => right _
-      | L2 => left eq_refl
-      | Pointer => right _
-      end
-    | Pointer => 
-      match y with
-      | Scratch8  => right _
-      | T0 => right _
-      | L0 => right _
-      | T1 => right _
-      | L1 => right _
-      | T2 => right _
-      | L2 => right _
-      | Pointer => left eq_refl
-      end
-    end
-  ); intros H; inversion H.
-  Defined.
-
-  Definition h16_eq_dec (x y: header 16) : {x = y} + {x <> y} :=
-    match x, y with 
-    | Scratch16, Scratch16 => left eq_refl
-    | _, _ => idProp
-    end.
-  Definition h24_eq_dec (x y: header 24) : {x = y} + {x <> y} :=
-    match x, y with 
-    | Scratch24, Scratch24 => left eq_refl
-    | _, _ => idProp
-    end.
-  Definition h32_eq_dec (x y: header 32) : {x = y} + {x <> y}.
-  refine (
-    match x, y with 
-    | Scratch32, Scratch32 => left eq_refl
-    | Timestamp, Timestamp => left eq_refl
-    | Timestamp, Scratch32 => right _
-    | Scratch32, Timestamp => right _
-    end
-  ); intros H; inversion H.
-  Defined.
-
-  Definition h40_eq_dec (x y: header 40) : {x = y} + {x <> y} :=
-    match x, y with 
-    | Scratch40, Scratch40 => left eq_refl
-    | _, _ => idProp
-    end.
-
-  Definition h48_eq_dec (x y: header 48) : {x = y} + {x <> y}.
-    refine (
-    match x with 
-    | V0 =>
-      match y with
-      | V0 => left eq_refl
-      | V1 => right _
-      | V2 => right _
-      end
-    | V1 =>
-      match y with
-      | V0 => right _
-      | V1 => left eq_refl
-      | V2 => right _
-      end
-    | V2 => 
-      match y with
-      | V0 => right _
-      | V1 => right _
-      | V2 => left eq_refl
-      end
-    end
-  ); intros H; inversion H.
-  Defined.
-
-  Definition header_eqdec_ (n: nat) (x: header n) (y: header n) : {x = y} + {x <> y}.
-    solve_header_eqdec_ n x y 
-      ((existT (fun n => forall x y: header n, {x = y} + {x <> y}) _ h8_eq_dec) :: 
-        (existT _ _ h16_eq_dec) :: (existT _ _ h24_eq_dec) :: (existT _ _ h32_eq_dec) :: 
-        (existT _ _ h40_eq_dec) :: (existT _ _ h48_eq_dec) :: (existT _ _ h4_eq_dec) :: nil).
-  Defined. 
-
-  Global Instance header_eqdec: forall n, EquivDec.EqDec (header n) eq := header_eqdec_.
-
-  Global Instance header_eqdec': EquivDec.EqDec (Syntax.H' header) eq.
+  Global Instance state_finite: @Finite state _ state_eq_dec.
   Proof.
-    solve_eqdec'.
+    solve_finiteness.
   Defined.
 
-  Global Instance header_finite: forall n, @Finite (header n) _ _.
+  Inductive header :=
+  | Scratch8
+  | Scratch16
+  | Scratch24
+  | Scratch32
+  | Scratch40
+  | T0
+  | L0
+  | V0
+  | T1
+  | L1
+  | V1
+  | T2
+  | L2
+  | V2
+  | Pointer
+  | Overflow
+  | Flag
+  | Timestamp.
+
+  Definition sz (h: header): nat :=
+    match h with
+    | Scratch8  => 8
+    | Scratch16  => 16
+    | Scratch24  => 24
+    | Scratch32  => 32
+    | Scratch40  => 40
+    | T0  => 8
+    | L0  => 8
+    | V0  => 48
+    | T1  => 8
+    | L1  => 8
+    | V1  => 48
+    | T2  => 8
+    | L2  => 8
+    | V2  => 48
+    | Pointer  => 8
+    | Overflow => 4
+    | Flag => 4
+    | Timestamp => 32
+    end.
+
+  Scheme Equality for header.
+  Global Instance header_eqdec: EquivDec.EqDec header eq := header_eq_dec.
+  Global Instance header_finite: @Finite header _ header_eq_dec.
   Proof.
-    intros n; solve_indexed_finiteness n [4; 8; 16; 24; 32; 40; 48].
-  Qed.
+    solve_finiteness.
+  Defined.
 
-  Global Program Instance header_finite': @Finite {n & header n} _ header_eqdec' :=
-    {| enum :=   [existT _ _ Scratch8 ;
-    existT _ _ Scratch16 ;
-    existT _ _ Scratch24 ;
-    existT _ _ Scratch32 ;
-    existT _ _ Scratch40 ;
-    existT _ _ T0 ;
-    existT _ _ L0 ;
-    existT _ _ V0 ;
-    existT _ _ T1 ;
-    existT _ _ L1 ;
-    existT _ _ V1 ;
-    existT _ _ T2 ;
-    existT _ _ L2 ;
-    existT _ _ V2 ;
-    existT _ _ Timestamp ;
-    existT _ _ Pointer ;
-    existT _ _ Overflow ;
-    existT _ _ Flag 
-    ]; |}.
-  Next Obligation.
-    solve_header_finite.
-  Qed.
-  Next Obligation.
-  dependent destruction X; subst;
-  repeat (
-    match goal with
-    | |- ?L \/ ?R => (now left; trivial) || right
-    end
-  ).
-  Qed.
-
-  Definition states (s: state) :=
+  Definition states (s: state) : Syntax.state state sz :=
     match s with
     | Parse0 =>
-      {| st_op := 
+      {| st_op :=
           extract(T0) ;;
           extract(L0) ;
-         st_trans := transition select (| EHdr T0, EHdr L0 |) {{
+         st_trans := transition select (| EHdr (sz := sz) T0, EHdr (sz := sz) L0 |) {{
            [| exact #b|0|1|0|0|0|1|0|0, exact #b|0|0|0|0|0|1|1|0 |] ==> inl Parse0S;;;
            [| exact #b|0|0|0|0|0|0|0|0, exact #b|0|0|0|0|0|0|0|0 |] ==> accept ;;;
            [| exact #b|0|0|0|0|0|0|0|1, exact #b|0|0|0|0|0|0|0|0 |] ==> accept ;;;
@@ -1586,43 +811,43 @@ Module TimestampSpec3.
          }}
       |}
     | Parse01 =>
-      {| st_op := 
+      {| st_op :=
           extract(Scratch8) ;;
-          V0 <- EConcat (m := 40) (EHdr Scratch8) ((EHdr V0)[48--8]) ;
+          V0 <- EConcat (m := 40) (EHdr (sz := sz) Scratch8) ((EHdr (sz := sz) V0)[48--8]) ;
          st_trans := transition inl Parse1;
       |}
     | Parse02 =>
-      {| st_op := 
+      {| st_op :=
           extract(Scratch16) ;;
-          V0 <- EConcat (m := 32) (EHdr Scratch16) ((EHdr V0)[48--16]) ;
+          V0 <- EConcat (m := 32) (EHdr (sz := sz) Scratch16) ((EHdr (sz := sz) V0)[48--16]) ;
          st_trans := transition inl Parse1;
       |}
     | Parse03 =>
-      {| st_op := 
+      {| st_op :=
           extract(Scratch24) ;;
-          V0 <- EConcat (m := 24) (EHdr Scratch24) ((EHdr V0)[48--24]) ;
+          V0 <- EConcat (m := 24) (EHdr (sz := sz) Scratch24) ((EHdr (sz := sz) V0)[48--24]) ;
          st_trans := transition inl Parse1;
       |}
     | Parse04 =>
-      {| st_op := 
+      {| st_op :=
           extract(Scratch32) ;;
-          V0 <- EConcat (m := 16) (EHdr Scratch32) ((EHdr V0)[48--32]) ;
+          V0 <- EConcat (m := 16) (EHdr (sz := sz) Scratch32) ((EHdr (sz := sz) V0)[48--32]) ;
          st_trans := transition inl Parse1;
       |}
     | Parse05 =>
-      {| st_op := 
+      {| st_op :=
           extract(Scratch40) ;;
-          V0 <- EConcat (m := 8) (EHdr Scratch40) ((EHdr V0)[48--40]) ;
+          V0 <- EConcat (m := 8) (EHdr (sz := sz) Scratch40) ((EHdr (sz := sz) V0)[48--40]) ;
          st_trans := transition inl Parse1;
       |}
     | Parse06 =>
-      {| st_op := 
+      {| st_op :=
           extract(V0) ;
          st_trans := transition inl Parse1;
       |}
 
     | Parse0S =>
-      {| st_op := 
+      {| st_op :=
           extract(Pointer) ;;
           extract(Overflow) ;;
           extract(Flag) ;;
@@ -1631,10 +856,10 @@ Module TimestampSpec3.
       |}
 
     | Parse1 =>
-      {| st_op := 
+      {| st_op :=
           extract(T1) ;;
           extract(L1) ;
-         st_trans := transition select (| EHdr T1, EHdr L1 |) {{
+         st_trans := transition select (| EHdr (sz := sz) T1, EHdr (sz := sz) L1 |) {{
            [| exact #b|0|1|0|0|0|1|0|0, exact #b|0|0|0|0|0|1|1|0 |] ==> inl Parse1S;;;
            [| exact #b|0|0|0|0|0|0|0|0, exact #b|0|0|0|0|0|0|0|0 |] ==> accept ;;;
            [| exact #b|0|0|0|0|0|0|0|1, exact #b|0|0|0|0|0|0|0|0 |] ==> accept ;;;
@@ -1648,42 +873,42 @@ Module TimestampSpec3.
          }}
       |}
     | Parse11 =>
-      {| st_op := 
+      {| st_op :=
           extract(Scratch8) ;;
-          V1 <- EConcat (m := 40) (EHdr Scratch8) ((EHdr V1)[48--8]) ;
+          V1 <- EConcat (m := 40) (EHdr (sz := sz) Scratch8) ((EHdr (sz := sz) V1)[48--8]) ;
          st_trans := transition inl Parse2;
       |}
     | Parse12 =>
-      {| st_op := 
+      {| st_op :=
           extract(Scratch16) ;;
-          V1 <- EConcat (m := 32) (EHdr Scratch16) ((EHdr V1)[48--16]) ;
+          V1 <- EConcat (m := 32) (EHdr (sz := sz) Scratch16) ((EHdr (sz := sz) V1)[48--16]) ;
          st_trans := transition inl Parse2;
       |}
     | Parse13 =>
-      {| st_op := 
+      {| st_op :=
           extract(Scratch24) ;;
-          V1 <- EConcat (m := 24) (EHdr Scratch24) ((EHdr V1)[48--24]) ;
+          V1 <- EConcat (m := 24) (EHdr (sz := sz) Scratch24) ((EHdr (sz := sz) V1)[48--24]) ;
          st_trans := transition inl Parse2;
       |}
     | Parse14 =>
-      {| st_op := 
+      {| st_op :=
           extract(Scratch32) ;;
-          V1 <- EConcat (m := 16) (EHdr Scratch32) ((EHdr V1)[48--32]) ;
+          V1 <- EConcat (m := 16) (EHdr (sz := sz) Scratch32) ((EHdr (sz := sz) V1)[48--32]) ;
          st_trans := transition inl Parse2;
       |}
     | Parse15 =>
-      {| st_op := 
+      {| st_op :=
           extract(Scratch40) ;;
-          V1 <- EConcat (m := 8) (EHdr Scratch40) ((EHdr V1)[48--40]) ;
+          V1 <- EConcat (m := 8) (EHdr (sz := sz) Scratch40) ((EHdr (sz := sz) V1)[48--40]) ;
          st_trans := transition inl Parse2;
       |}
     | Parse16 =>
-      {| st_op := 
+      {| st_op :=
           extract(V1) ;
          st_trans := transition inl Parse2;
       |}
     | Parse1S =>
-      {| st_op := 
+      {| st_op :=
           extract(Pointer) ;;
           extract(Overflow) ;;
           extract(Flag) ;;
@@ -1692,10 +917,10 @@ Module TimestampSpec3.
       |}
 
     | Parse2 =>
-      {| st_op := 
+      {| st_op :=
           extract(T2) ;;
           extract(L2) ;
-         st_trans := transition select (| EHdr T2, EHdr L2 |) {{
+         st_trans := transition select (| EHdr (sz := sz) T2, EHdr (sz := sz) L2 |) {{
            [| exact #b|0|1|0|0|0|1|0|0, exact #b|0|0|0|0|0|1|1|0 |] ==> inl Parse2S;;;
            [| exact #b|0|0|0|0|0|0|0|0, exact #b|0|0|0|0|0|0|0|0 |] ==> accept ;;;
            [| exact #b|0|0|0|0|0|0|0|1, exact #b|0|0|0|0|0|0|0|0 |] ==> accept ;;;
@@ -1709,42 +934,42 @@ Module TimestampSpec3.
          }}
       |}
     | Parse21 =>
-      {| st_op := 
+      {| st_op :=
           extract(Scratch8) ;;
-          V1 <- EConcat (m := 40) (EHdr Scratch8) ((EHdr V2)[48--8]) ;
+          V1 <- EConcat (m := 40) (EHdr (sz := sz) Scratch8) ((EHdr (sz := sz) V2)[48--8]) ;
          st_trans := transition accept;
       |}
     | Parse22 =>
-      {| st_op := 
+      {| st_op :=
           extract(Scratch16) ;;
-          V2 <- EConcat (m := 32) (EHdr Scratch16) ((EHdr V2)[48--16]) ;
+          V2 <- EConcat (m := 32) (EHdr (sz := sz) Scratch16) ((EHdr (sz := sz) V2)[48--16]) ;
          st_trans := transition accept;
       |}
     | Parse23 =>
-      {| st_op := 
+      {| st_op :=
           extract(Scratch24) ;;
-          V2 <- EConcat (m := 24) (EHdr Scratch24) ((EHdr V2)[48--24]) ;
+          V2 <- EConcat (m := 24) (EHdr (sz := sz) Scratch24) ((EHdr (sz := sz) V2)[48--24]) ;
          st_trans := transition accept;
       |}
     | Parse24 =>
-      {| st_op := 
+      {| st_op :=
           extract(Scratch32) ;;
-          V2 <- EConcat (m := 16) (EHdr Scratch32) ((EHdr V2)[48--32]) ;
+          V2 <- EConcat (m := 16) (EHdr (sz := sz) Scratch32) ((EHdr (sz := sz) V2)[48--32]) ;
          st_trans := transition accept;
       |}
     | Parse25 =>
-      {| st_op := 
+      {| st_op :=
           extract(Scratch40) ;;
-          V2 <- EConcat (m := 8) (EHdr Scratch40) ((EHdr V2)[48--40]) ;
+          V2 <- EConcat (m := 8) (EHdr (sz := sz) Scratch40) ((EHdr (sz := sz) V2)[48--40]) ;
          st_trans := transition accept;
       |}
     | Parse26 =>
-      {| st_op := 
+      {| st_op :=
           extract(V2) ;
          st_trans := transition accept;
       |}
     | Parse2S =>
-      {| st_op := 
+      {| st_op :=
           extract(Pointer) ;;
           extract(Overflow) ;;
           extract(Flag) ;;
@@ -1753,9 +978,9 @@ Module TimestampSpec3.
       |}
     end.
 
-  Program Definition aut: Syntax.t state header :=
+  Program Definition aut: Syntax.t state sz :=
     {| t_states := states |}.
-  Solve Obligations with (destruct s; cbv; Lia.lia).
+  Solve Obligations with (destruct s || destruct h; cbv; Lia.lia).
 
 End TimestampSpec3.
 
